lots of changes from box to low* box. first commit

secure_api/box/Box.Key.fst
@@ -13,12 +13,11 @@ open Crypto.Symmetric.Bytes
 open Box.Flags
 
 module ID = Box.Index
-module Plain = Box.Plain
 module MR = FStar.Monotonic.RRef
 module HH = FStar.HyperHeap
 module HS = FStar.HyperStack
 module MM = MonotoneMap
-module SPEC = Spec.SecretBox
+module Plain = Box.Plain
 
 assume val is_random: bytes -> Type0
 
@@ -29,22 +28,25 @@ let id = ID.id
 type log_region =
   r:MR.rid{is_eternal_region r}
 
-type key_t (im:index_module) (pm:plain_module)= Type0
+let key_raw (kpm:plain_module) = Plain.plain_bytes kpm
 
-//type aes_key = SPEC.key
-//type cipher = b:bytes{Seq.length b >= 16 /\ (Seq.length b - 16) / Spec.Salsa20.blocklen < pow2 32}
-//noeq type key_t2 (im:index_module) =
+let check_length (max_length:nat) (n:nat) : GTot bool = n = max_length
 
 #set-options "--z3rlimit 300 --max_ifuel 1 --max_fuel 0"
+#set-options "--__temp_no_proj Box.Key"
 abstract noeq type key_module (im:index_module) =
   | KM:
     keylen: nat ->
-    key_type: (im':index_module{im' == im} -> t:Type0) ->
-    get_index: (k:key_type im -> i:id im) -> // You have to have faith in this function...
-    get_rawGT: ((k:key_type im) -> GTot (b:lbytes keylen)) -> // You have to have faith in this function...
-    invariant: (h:mem -> Type0) ->
+    key_type: (i:id im -> t:Type0) ->
+    kpm:plain_module{Plain.valid_length kpm == (check_length keylen)} ->
+    get_rawGT: (i:id im -> (k:key_type i) -> GTot (raw:key_raw kpm)) -> // You have to have faith in this function...
+    invariant: (h:mem -> t:Type0) -> // Invariant should still hold if only the top of the stack was touched
+    invariant_framing_lemma: (h0:mem -> h1:mem -> Lemma
+      (requires (invariant h0))
+      (ensures ((modifies_one h0.tip h0 h1 /\ h0.tip <> root) ==> invariant h1))
+    ) ->
     key_log_region: (rgn:log_region{disjoint rgn (ID.get_rgn im)}) ->
-    gen: (i:id im -> ST (k:key_type im{get_index k = i}) // The spec should indicate that the result is random and that gen is idempotent
+    gen: (i:id im -> ST (k:key_type i) // The spec should indicate that the result is random and that gen is idempotent
       (requires (fun h0 ->
         (ID.fresh im i h0 \/ ID.honest im i)
         /\ invariant h0))
@@ -52,32 +54,31 @@ abstract noeq type key_module (im:index_module) =
         invariant h1
         /\ modifies (Set.singleton key_log_region) h0 h1
         ))) ->
-    set: ((i:id im {Game3? current_game \/ Game0? current_game}) -> (b:lbytes keylen) -> (k:key_type im{get_index k = i /\ b = get_rawGT k})) ->
-    coerce: (i:id im{ID.dishonest im i} -> raw:lbytes keylen -> (k:key_type im{get_index k = i /\ raw=get_rawGT k})) ->
-    leak: (k:key_type im{ID.dishonest im (get_index k)} -> (raw:lbytes keylen{raw = get_rawGT k})) ->
+    set: ((i:id im {~(Game2? current_game)}) -> (raw:key_raw kpm) -> (k:key_type i{raw == get_rawGT i k})) ->
+    coerce: (i:id im{ID.dishonest im i} -> (raw:key_raw kpm) -> (k:key_type i{raw == get_rawGT i k})) ->
+    leak: (i:id im{ID.dishonest im i} -> k:key_type i -> (raw:key_raw kpm)) ->
     key_module im
 
-val get_keylen: im:index_module -> km:key_module im -> n:nat{n = km.keylen}
-let get_keylen im km =
+val get_keylen: #im:index_module -> km:key_module im -> n:nat{n = km.keylen}
+let get_keylen #im km =
   km.keylen
 
-val get_keytype: im:index_module -> km:key_module im -> t:Type0{t == km.key_type im}
-let get_keytype im km =
-  km.key_type im
+val get_keytype: #im:index_module -> km:key_module im -> t:(i:id im -> Type0)
+let get_keytype #im km =
+  km.key_type
 
-val get_index: im:index_module -> km:key_module im -> gi:(k:km.key_type im -> i:id im){gi==km.get_index}
-let get_index im km =
-  km.get_index
+val get_pm: #im:index_module -> km:key_module im -> pm:plain_module{pm == km.kpm}
+let get_pm #im km = km.kpm
 
-val get_rawGT: im:index_module -> km:key_module im -> gr:(k:km.key_type im -> GTot (b:lbytes km.keylen)){gr == km.get_rawGT}
-let get_rawGT im km =
+val get_rawGT: #im:index_module -> km:key_module im -> gr:(i:id im -> k:km.key_type i -> GTot (b:key_raw km.kpm)){gr == km.get_rawGT}
+let get_rawGT #im km =
   km.get_rawGT
 
-val get_log_region: im:index_module -> km:key_module im -> rgn:log_region{rgn = km.key_log_region}
-let get_log_region im km =
+val get_log_region: #im:index_module -> km:key_module im -> rgn:log_region{rgn = km.key_log_region}
+let get_log_region #im km =
   km.key_log_region
 
-val gen: (im:index_module) -> (km:key_module im) -> (i:id im) -> ST (k:km.key_type im{km.get_index k = i})
+val gen: (#im:index_module) -> (km:key_module im) -> (i:id im) -> ST (k:km.key_type i)
   (requires (fun h0 ->
     (ID.fresh im i h0 \/ ID.honest im i)
     /\ km.invariant h0))
@@ -85,34 +86,44 @@ val gen: (im:index_module) -> (km:key_module im) -> (i:id im) -> ST (k:km.key_ty
     km.invariant h1
     /\ modifies (Set.singleton km.key_log_region) h0 h1
   ))
-let gen im km i =
+let gen #im km i =
   km.gen i
 
-val set: (im:index_module) -> (km:key_module im) -> (i:id im {~(Game2? current_game)}) -> (b:lbytes km.keylen) -> (k:km.key_type im{km.get_index k = i /\ b = km.get_rawGT k})
-let set im km i b =
+val set: (#im:index_module) -> (km:key_module im) -> (i:id im {~(Game2? current_game)}) -> (b:key_raw km.kpm) -> (k:km.key_type i{b == km.get_rawGT i k})
+let set #im km i b =
   km.set i b
 
-val coerce: (im:index_module) -> (km:key_module im) -> (i:id im{ID.dishonest im i}) -> (b:lbytes km.keylen) -> (k:km.key_type im{km.get_index k = i /\ b = km.get_rawGT k})
-let coerce im km i b =
+val coerce: (#im:index_module) -> (km:key_module im) -> (i:id im{ID.dishonest im i}) -> (b:key_raw km.kpm) -> (k:km.key_type i{b == km.get_rawGT i k})
+let coerce #im km i b =
   km.coerce i b
 
-val leak: im:index_module -> (km:key_module im) -> (k:km.key_type im{ID.dishonest im (km.get_index k)}) -> (b:lbytes km.keylen{b=km.get_rawGT k})
-let leak im km k =
+val leak: #im:index_module -> (km:key_module im) -> i:id im{ID.dishonest im i} -> (k:km.key_type i) -> (b:key_raw km.kpm)
+let leak #im km k =
   km.leak k
 
-val invariant: im:index_module -> km:key_module im -> inv:(h0:mem -> Type0){inv == km.invariant}
-let invariant im km =
+val invariant: #im:index_module -> km:key_module im -> inv:(h0:mem -> Type0){inv == km.invariant}
+let invariant #im km =
   km.invariant
+
+val invariant_framing_lemma: #im:index_module -> km:key_module im -> h0:mem -> h1:mem -> Lemma
+  (requires (km.invariant h0))
+  (ensures ((modifies_one h0.tip h0 h1 /\ h0.tip <> root) ==> km.invariant h1))
+let invariant_framing_lemma #im km h0 h1 =
+  km.invariant_framing_lemma h0 h1
 
 #set-options "--z3rlimit 2000 --max_ifuel 2 --max_fuel 0"
 val create: (im:index_module) ->
             (keylen: nat) ->
-            (km_key_type: (im':index_module{im' == im} -> t:Type0)) ->
-            (km_get_index: (k:km_key_type im -> i:id im)) -> // You have to have faith in this function...
-            (km_get_rawGT: ((k:km_key_type im) -> GTot (b:lbytes keylen))) -> // You have to have faith in this function...
+            (km_key_type: (i:id im -> t:Type0)) ->
+            (km_kpm:plain_module{Plain.valid_length km_kpm == (check_length keylen)}) ->
+            (km_get_rawGT: ((i:id im) -> (k:km_key_type i) -> GTot (raw:key_raw km_kpm))) -> // You have to have faith in this function...
             (km_invariant: (h:mem -> Type0)) ->
+            (km_invariant_framing_lemma: (h0:mem -> h1:mem -> Lemma
+              (requires (km_invariant h0))
+              (ensures ((modifies_one h0.tip h0 h1 /\ h0.tip <> root) ==> km_invariant h1))
+            )) ->
             (km_key_log_region: (r:log_region{disjoint r (ID.get_rgn im)})) ->
-            (km_gen: (i:id im -> ST (k:km_key_type im{km_get_index k = i}) // The spec should indicate that the result is random and that gen is idempotent
+            (km_gen: (i:id im -> ST (k:km_key_type i) // The spec should indicate that the result is random and that gen is idempotent
               (requires (fun h0 ->
                 (ID.fresh im i h0 \/ ID.honest im i)
                 /\ km_invariant h0))
@@ -120,17 +131,18 @@ val create: (im:index_module) ->
                 km_invariant h1
                 /\ modifies (Set.singleton km_key_log_region) h0 h1
               )))) ->
-            (km_set: (i:id im {Game3? current_game \/ Game0? current_game} -> b:lbytes keylen -> (k:km_key_type im{km_get_index k = i /\ b = km_get_rawGT k}))) ->
-            (km_coerce: (i:id im{ID.dishonest im i} -> raw:lbytes keylen -> (k:km_key_type im{km_get_index k = i /\ raw=km_get_rawGT k}))) ->
-            (km_leak: (k:km_key_type im{ID.dishonest im (km_get_index k)} -> (raw:lbytes keylen{raw = km_get_rawGT k}))) ->
+            (km_set: (i:id im{~(Game2? current_game)} -> raw:key_raw km_kpm -> (k:km_key_type i{raw == km_get_rawGT i k}))) ->
+            (km_coerce: (i:id im{ID.dishonest im i} -> raw:key_raw km_kpm -> (k:km_key_type i{raw == km_get_rawGT i k}))) ->
+            (km_leak: (i:id im{ID.dishonest im i} -> k:km_key_type i -> (raw:key_raw km_kpm))) ->
             (km:key_module im{
-              get_keytype im km == km_key_type im
-              /\ get_keylen im km == keylen
-              /\ get_index im km == km_get_index
-              /\ get_rawGT im km == km_get_rawGT
-              /\ invariant im km == km_invariant
-              /\ get_log_region im km == km_key_log_region
+              keylen == km.keylen
+              /\ get_pm km == km_kpm
+              /\ get_keytype km == km_key_type
+              /\ get_keylen km == keylen
+              /\ get_rawGT km == km_get_rawGT
+              /\ invariant km == km_invariant
+              /\ get_log_region km == km_key_log_region
     })
-let create im keylen km_key_type km_get_index km_get_rawGT km_invariant km_key_log_region km_gen km_set km_coerce km_leak =
-  let km = KM keylen km_key_type km_get_index km_get_rawGT km_invariant km_key_log_region km_gen km_set km_coerce km_leak in
+let create im keylen km_key_type kpm km_get_rawGT km_invariant km_invariant_framing_lemma km_key_log_region km_gen km_set km_coerce km_leak =
+  let km = KM keylen km_key_type kpm km_get_rawGT km_invariant km_invariant_framing_lemma km_key_log_region km_gen km_set km_coerce km_leak in
   km
