secure_api/box/Box.ODH.fst
@@ -35,25 +35,33 @@ let smaller om i1 i2 = smaller' om.dh_share_length i1 i2
 
 //let share_from_exponent' dh_exp = Curve.scalarmult dh_exp Curve.base_point
 
-let hash_fun om = om.hash
-let dh_exponentiate om = om.exponentiate
-let share_from_exponent om exp = om.exponentiate exp om.base_point
+let hash_fun #om = om.hash_low
+let dh_exponentiate #om = om.exponentiate_low
+
+//val share_from_exponent: #om:odh_module -> exp:dh_exponent om -> ST (sh:dh_share om)
+//      (requires (fun h0 -> True))
+//      (ensures (fun h0 res h1 ->
+//        Plain.plain_to_bytesGT h1 res == om.exponentiate (Plain.plain_to_bytesGT h1 exp) om.base_point
+//        /\ modifies_none h0 h1
+//      ))
+let share_from_exponent #om exp = om.exponentiate_low exp (get_base_point_low om)
+let share_from_exponent_bytes #om exp = om.exponentiate exp (om.base_point)
 
 noeq abstract type pkey' (om:odh_module) =
-  | PKEY: pk_share:dh_share om-> pkey' om
+  | PKEY: pk_share:dh_share_bytes om -> pkey' om
+
+//noeq abstract type skey' (om:odh_module) =
+//  | SKEY: sk_exp:dh_exponent om -> pk:pkey' om{Plain.plain_to_bytesGT spm pk.pk_share == om.exponentiate (Plain.plain_to_bytesGT om.epm sk_exp) om.base_point} -> skey' om
 
 noeq abstract type skey' (om:odh_module) =
-  | SKEY: sk_exp:dh_exponent om -> pk:pkey' om{pk.pk_share = om.exponentiate sk_exp om.base_point} -> skey' om
+  | SKEY: sk_exp:dh_exponent_bytes om -> pk:pkey' om -> skey' om
 
 let skey = skey'
 let pkey = pkey'
 
-let get_pkey om sk = sk.pk
+let get_pkey #om sk = sk.pk
 
 #set-options "--z3rlimit 300 --max_ifuel 1 --max_fuel 0"
-let compatible_keys om sk pk =
-  sk.pk =!= pk
-
 let get_hash_length om = om.hash_length
 let get_dh_share_length om = om.dh_share_length
 let get_dh_exponent_length om = om.dh_exponent_length
@@ -61,44 +69,52 @@ let get_base_point om = om.base_point
 let get_index_module om = om.im
 let get_key_index_module om = om.kim
 let get_key_module om kim = om.km
+let get_kpm om = om.kpm
+let get_spm om = om.spm
+let get_epm om = om.epm
 
 #set-options "--z3rlimit 300 --max_ifuel 0 --max_fuel 0"
-let total_order_lemma om i1 i2 =
-  let i1:dh_share om = i1 in
-  let i2:dh_share om = i2 in
+let total_order_lemma #om i1 i2 =
+  let i1:dh_share_bytes om = i1 in
+  let i2:dh_share_bytes om = i2 in
   LE.lemma_little_endian_bij i1 i2
 
 #set-options "--z3rlimit 300 --max_ifuel 1 --max_fuel 0"
-let create hash_len dh_share_len dh_exp_len hash_fun exponentiate base_point im kim km rgn =
-  ODH rgn hash_len dh_share_len dh_exp_len hash_fun exponentiate base_point im kim km
+let create hash_len dh_share_len dh_exp_len kpm spm epm hash hash_low exponentiate exponentiate_low base_point im kim km rgn =
+  ODH rgn hash_len dh_share_len dh_exp_len kpm spm epm hash hash_low exponentiate exponentiate_low base_point im kim km
 
-let pk_get_share om k = k.pk_share
+let pk_get_share_bytesGT #om k = k.pk_share
 
-let lemma_pk_get_share_inj om pk = ()
+let pk_get_share #om k = Plain.bytes_to_plainST om.spm k.pk_share
 
-let get_skeyGT om sk =
+let get_skeyGT #om sk =
   sk.sk_exp
 
-let sk_get_share om sk =
-  sk.pk.pk_share
+let sk_get_share_bytesGT #om sk = sk.pk.pk_share
+
+let sk_get_share #om sk =
+  Plain.bytes_to_plainST om.spm sk.pk.pk_share
+
+let compatible_keys #om sk pk =
+  pk_get_share_bytesGT #om pk =!= sk_get_share_bytesGT sk
 
 #set-options "--z3rlimit 300 --max_ifuel 1 --max_fuel 0"
-let leak_skey om sk =
+let leak_skey #om sk =
   sk.sk_exp
 
 assume val boundless_random_bytes: n:nat -> lbytes n
 
-let keygen om =
+let keygen #om =
   let dh_exponent = boundless_random_bytes om.dh_exponent_length in
-  let dh_pk = PKEY (share_from_exponent om dh_exponent) in
+  let dh_pk = PKEY (share_from_exponent_bytes dh_exponent) in
   let dh_sk = SKEY dh_exponent dh_pk in
   dh_pk,dh_sk
 
-let coerce_pkey om dh_sh =
+let coerce_pkey #om dh_sh =
   PKEY dh_sh
 
-let coerce_keypair om dh_ex =
-  let dh_sh = share_from_exponent om dh_ex in
+let coerce_keypair #om dh_ex =
+  let dh_sh = share_from_exponent_bytes #om dh_ex in
   let pk = PKEY dh_sh in
   let sk = SKEY dh_ex pk in
   pk,sk
@@ -108,19 +124,40 @@ let compose_ids om s1 s2 =
      let i = (s1,s2) in
      i
   else
-    (total_order_lemma om s1 s2;
+    (total_order_lemma s1 s2;
     let i = (s2,s1) in
     i)
 
-let prf_odhGT om sk pk =
-  let raw_k = (dh_exponentiate om) sk.sk_exp pk.pk_share in
-  let k = (hash_fun om) raw_k in
+let prf_odhGT #om sk pk =
+  let raw_k = om.exponentiate sk.sk_exp pk.pk_share in
+  let k = om.hash raw_k in
   k
 
 let lemma_shares om sk = ()
 
+#set-options "--z3rlimit 1000 --max_ifuel 1 --max_fuel 0"
+val prf_odh: om:odh_module -> sk:skey om -> pk:pkey om{compatible_keys sk pk} -> StackInline (k:(Key.get_keytype #om.kim om.km) (compose_ids om (pk_get_share_bytesGT pk) (sk_get_share_bytesGT sk)))
+  (requires (fun h0 ->
+    let i = compose_ids om (pk_get_share_bytesGT pk) (sk_get_share_bytesGT sk) in
+    ID.registered om.kim i
+    /\ Key.invariant om.km h0
+  ))
+  (ensures (fun h0 k h1 ->
+    let i = compose_ids om (pk_get_share_bytesGT pk) (sk_get_share_bytesGT sk) in
+    let raw = Key.get_rawGT #om.kim om.km i k in
+    ((ID.honest om.kim i /\ b2t Flags.prf_odh) ==>
+        modifies (Set.singleton (Key.get_log_region om.km)) h0 h1)
+    // We should guarantee, that the key is randomly generated. Generally, calls to prf_odh should be idempotent. How to specify that?
+    // Should we have a genPost condition that we guarantee here?
+    /\ ((ID.dishonest om.kim i \/ ~(b2t Flags.prf_odh)) ==>
+        (Plain.plain_to_bytesGT h1 raw == ((prf_odhGT sk pk)) // Functional correctness.
+        /\ modifies_none h0 h1))
+    /\ (modifies (Set.singleton (Key.get_log_region om.km))h0 h1 \/ modifies_none h0 h1)
+    /\ Key.invariant om.km h1
+  ))
 
 let prf_odh om sk pk =
+  let h0 = get() in
   let i1 = pk.pk_share in
   let i2 = sk.pk.pk_share in
   let i = compose_ids om i1 i2 in
@@ -130,12 +167,29 @@ let prf_odh om sk pk =
   let honest_i = ID.get_honest om.kim i in
   match honest_i && Flags.prf_odh with
   | true ->
-    let k = Key.gen om.kim om.km i in
+    let k = Key.gen om.km i in
+    let h1 = get() in
+    Key.invariant_framing_lemma om.km h0 h1;
     k
   | false ->
-    let raw_k = om.exponentiate sk.sk_exp pk.pk_share in
-    let hashed_raw_k = om.hash raw_k in
+    let h0 = get() in
+    let raw_sk = Plain.bytes_to_plainST om.epm (leak_skey sk) in
+    let h1 = get() in
+    assert(Key.invariant om.km h1);
+    admit();
+    let raw_k = om.exponentiate_low raw_sk (pk_get_share pk) in
+    let hashed_raw_k = om.hash_low raw_k in
     if not honest_i then
-      Key.coerce om.kim om.km i hashed_raw_k
+      let h1 = get() in
+      Key.invariant_framing_lemma om.km h0 h1;
+      assert((ID.dishonest om.kim i \/ ~(b2t Flags.prf_odh)));
+      let h1 = get() in
+      assert(Key.invariant om.km h1);
+      admit();
+      Key.coerce om.km i hashed_raw_k
     else
-      Key.set om.kim om.km i hashed_raw_k
+      let h1 = get() in
+      Key.invariant_framing_lemma om.km h0 h1;
+      //assert(~(ID.dishonest om.kim i \/ ~(b2t Flags.prf_odh)));
+      admit();
+      Key.set om.km i hashed_raw_k
