secure_api/box/Box.ODH.fsti
@@ -12,81 +12,157 @@ module HH = FStar.HyperHeap
 module Key = Box.Key
 
 val smaller': n:nat -> i1:lbytes n -> i2:lbytes n -> b:bool{b ==> i1 <> i2}
+let plain_module = Plain.plain_module
+
+let plain (pm:plain_module) = Plain.plain pm
+let plain_bytes (pm:plain_module) = b:bytes{Plain.valid_length pm (Seq.length b)}
 
 #set-options "--__temp_no_proj Box.ODH"
 #set-options "--z3rlimit 300 --max_ifuel 2 --max_fuel 0"
 abstract noeq type odh_module = // require subId type to be dh_share?
   | ODH:
     rgn:(r:HH.rid) ->
-    hash_length:(n:nat) ->
-    dh_share_length:(n:nat) ->
-    dh_exponent_length:(n:nat) ->
+    hash_length:(n:nat{0 < n /\ n <= UInt.max_int 32}) ->
+    dh_share_length:(n:nat{0 < n /\ n <= UInt.max_int 32}) ->
+    dh_exponent_length:(n:nat{0 < n /\ n <= UInt.max_int 32}) ->
+    kpm:plain_module{Plain.valid_length kpm == Key.check_length hash_length} ->
+    spm:plain_module{Plain.valid_length spm == Key.check_length dh_share_length} ->
+    epm:plain_module{Plain.valid_length epm == Key.check_length dh_exponent_length} ->
     hash: (lbytes dh_share_length -> (lbytes hash_length)) ->
-    exponentiate: (lbytes dh_exponent_length -> lbytes dh_share_length -> Tot (lbytes dh_share_length)) ->
+    hash_low: (input:plain spm -> ST (output:plain kpm)
+      (requires (fun h0 -> True))
+      (ensures (fun h0 output h1 ->
+        Plain.plain_to_bytesGT h1 output == hash (Plain.plain_to_bytesGT h1 input)
+        /\ modifies_none h0 h1
+      ))
+    ) ->
+    exponentiate: (e:lbytes dh_exponent_length -> sh:lbytes dh_share_length -> Tot (lbytes dh_share_length)) ->
+    exponentiate_low: (e:plain epm -> sh:plain spm -> ST (res:plain spm)
+      (requires (fun h0 -> True))
+      (ensures (fun h0 res h1 ->
+        Plain.plain_to_bytesGT h1 res == exponentiate (Plain.plain_to_bytesGT h1 e) (Plain.plain_to_bytesGT h1 sh)
+        /\ modifies_none h0 h1
+      ))
+    ) ->
     base_point: lbytes dh_share_length ->
+    //base_point_low: plain spm{Plain.plain_to_bytesGT spm h1 base_point_low == base_point} ->
     im:ID.index_module{ID.id im == lbytes dh_share_length} ->
-    kim:ID.index_module{ID.id kim == i:(lbytes dh_share_length * lbytes dh_share_length){b2t (smaller' dh_share_length (fst i) (snd i))}} ->
-    km:Key.key_module kim{Key.get_keylen kim km = hash_length} ->
+    kim:ID.index_module{ID.id kim == i:(plain_bytes spm * plain_bytes spm){b2t (smaller' dh_share_length (fst i) (snd i))}} ->
+    km:Key.key_module kim{Key.get_keylen km = hash_length /\ Key.get_pm km == kpm} ->
     odh_module
 
 val smaller: om:odh_module -> i1:lbytes om.dh_share_length -> i2:lbytes om.dh_share_length -> b:bool{b == smaller' om.dh_share_length i1 i2}
 
+let get_base_point_low om =
+  Plain.bytes_to_plainST om.spm om.base_point
+
 #set-options "--z3rlimit 1000 --max_ifuel 2 --max_fuel 0"
 // Basic types
-let dh_share (om:odh_module) = lbytes om.dh_share_length
-let dh_exponent (om:odh_module) = lbytes om.dh_exponent_length
-let hash_output (om:odh_module) = lbytes om.hash_length
-let key_id (om:odh_module) =  i:(dh_share om * dh_share om){b2t (smaller om (fst i) (snd i))}
-val hash_fun: om:odh_module -> (hash:(dh_share om -> (hash_output om)){hash == om.hash})
-val dh_exponentiate: om:odh_module -> exp:(dh_exponent om -> dh_share om -> (dh_share om)){exp == om.exponentiate}
-val share_from_exponent: om:odh_module -> exp:dh_exponent om -> Tot (sh:dh_share om{sh = om.exponentiate exp om.base_point})
+let dh_share (om:odh_module) = plain om.spm
+let dh_share_bytes (om:odh_module) = plain_bytes om.spm
+let dh_exponent (om:odh_module) = plain om.epm
+let dh_exponent_bytes (om:odh_module) = plain_bytes om.epm
+let hash_output (om:odh_module) = plain om.kpm
+let hash_output_bytes (om:odh_module) = plain_bytes om.kpm
+let key_id (om:odh_module) =  i:(dh_share_bytes om * dh_share_bytes om){b2t (smaller om (fst i) (snd i))}
+
+val hash_fun: #om:odh_module -> hash:(input:dh_share om -> ST (hash_output om)
+      (requires (fun h0 -> True))
+      (ensures (fun h0 output h1 ->
+        Plain.plain_to_bytesGT h1 output == om.hash (Plain.plain_to_bytesGT h1 input)
+        /\ modifies_none h0 h1
+      ))){hash == om.hash_low}
+
+val dh_exponentiate: #om:odh_module -> exp:(e:dh_exponent om -> sh:dh_share om -> ST (res:dh_share om)
+      (requires (fun h0 -> True))
+      (ensures (fun h0 res h1 ->
+        Plain.plain_to_bytesGT h1 res == om.exponentiate (Plain.plain_to_bytesGT h1 e) (Plain.plain_to_bytesGT h1 sh)
+        /\ modifies_none h0 h1
+      ))
+    ){exp == om.exponentiate_low}
+
+//val share_from_exponent: #om:odh_module -> exp:dh_exponent om -> ST (sh:dh_share om)
+//      (requires (fun h0 -> True))
+//      (ensures (fun h0 res h1 ->
+//        Plain.plain_to_bytesGT h1 res == om.exponentiate (Plain.plain_to_bytesGT h1 exp) om.base_point
+//        /\ modifies_none h0 h1
+//      ))
 
 // Key types and key handling
 val skey: om:odh_module -> Type0
 val pkey: om:odh_module -> Type0
-val get_pkey: om:odh_module -> skey om -> pkey om
-val compatible_keys: om:odh_module -> sk:skey om -> pk:pkey om -> t:Type0{t <==> pk =!= get_pkey om sk}
+val get_pkey: #om:odh_module -> skey om -> pkey om
+//val get_pkey_bytesGT: om:odh_module -> skey om -> GTot (pkey om)
+
+//val compatible_keys_lemma: om:odh_module -> sk:skey om -> pk:pkey om -> Lemma
+//  (requires (compatible_keys om sk pk))
+//  (ensures (compatible_keys om sk pk ==> (Plain.plain_to_bytesGT om.spm pk) =!= Plain.plain_to_bytesGT om.spm (get_pkey om sk)))
+
 
 // Getters
 val get_hash_length: om:odh_module -> n:nat{n = om.hash_length}
 val get_dh_share_length: om:odh_module -> n:nat{n = om.dh_share_length}
 val get_dh_exponent_length: om:odh_module -> n:nat{n = om.dh_exponent_length}
-val get_base_point: om:odh_module -> sh:dh_share om{sh = om.base_point}
+val get_base_point: om:odh_module -> sh:dh_share_bytes om{sh == om.base_point}
 val get_index_module: om:odh_module -> im:ID.index_module{im==om.im}
 val get_key_index_module: om:odh_module -> kim:ID.index_module{kim==om.kim}
-val get_key_module: om:odh_module -> kim:ID.index_module{kim == om.kim} -> km:Key.key_module kim{km==om.km /\ Key.get_keylen kim km = om.hash_length}
+val get_key_module: om:odh_module -> kim:ID.index_module{kim == om.kim} -> km:Key.key_module kim{km==om.km /\ Key.get_keylen km = om.hash_length}
+val get_kpm: om:odh_module -> kpm:plain_module{kpm == om.kpm}
+val get_spm: om:odh_module -> spm:plain_module{spm == om.spm}
+val get_epm: om:odh_module -> epm:plain_module{epm == om.epm}
 
-val total_order_lemma: (om:odh_module -> i1:dh_share om -> i2:dh_share om -> Lemma
+val total_order_lemma: (#om:odh_module -> i1:dh_share_bytes om -> i2:dh_share_bytes om -> Lemma
   (requires True)
   (ensures
     (b2t (smaller om i1 i2) ==> (forall i. i <> i1 /\ i <> i2 /\ b2t (smaller om i i1) ==> b2t (smaller om i i2)))
     /\ (~ (b2t (smaller om i1 i2)) <==> (i1 = i2 \/ b2t (smaller om i2 i1)))))
 
 #set-options "--z3rlimit 300 --max_ifuel 2 --max_fuel 1"
-val create: om_hash_len:nat ->
-            om_dh_share_len:nat ->
-            om_dh_exponent_len:nat ->
-            om_hash_fun: (lbytes om_dh_share_len -> (lbytes om_hash_len)) ->
-            om_exponentiate: (lbytes om_dh_exponent_len -> lbytes om_dh_share_len -> (lbytes om_dh_share_len)) ->
-            om_base_point: lbytes om_dh_share_len ->
-            om_im:ID.index_module{ID.id om_im == lbytes om_dh_share_len} ->
-            om_kim:ID.index_module{ID.id om_kim == i:(lbytes om_dh_share_len * lbytes om_dh_share_len){b2t (smaller' om_dh_share_len (fst i) (snd i))}} ->
-            om_km:Key.key_module om_kim{Key.get_keylen om_kim om_km = om_hash_len} ->
+val create: om_hash_length:nat{ 0 < om_hash_length /\ om_hash_length <= UInt.max_int 32} ->
+            om_dh_share_length:nat{0 < om_dh_share_length /\ om_dh_share_length <= UInt.max_int 32} ->
+            om_dh_exponent_length:nat{0 < om_dh_exponent_length /\ om_dh_exponent_length <= UInt.max_int 32} ->
+            om_kpm:plain_module{Plain.valid_length om_kpm == Key.check_length om_hash_length} ->
+            om_spm:plain_module{Plain.valid_length om_spm == Key.check_length om_dh_share_length} ->
+            om_epm:plain_module{Plain.valid_length om_epm == Key.check_length om_dh_exponent_length} ->
+            om_hash: (lbytes om_dh_share_length -> (lbytes om_hash_length)) ->
+            om_hash_low: (input:plain om_spm -> ST (output:plain om_kpm)
+              (requires (fun h0 -> True))
+              (ensures (fun h0 output h1 ->
+                Plain.plain_to_bytesGT h1 output == om_hash (Plain.plain_to_bytesGT h1 input)
+                /\ modifies_none h0 h1
+              ))
+            ) ->
+            om_exponentiate: (e:lbytes om_dh_exponent_length -> sh:lbytes om_dh_share_length -> Tot (lbytes om_dh_share_length)) ->
+            om_exponentiate_low: (e:plain om_epm -> sh:plain om_spm -> ST (res:plain om_spm)
+              (requires (fun h0 -> True))
+              (ensures (fun h0 res h1 ->
+                Plain.plain_to_bytesGT h1 res == om_exponentiate (Plain.plain_to_bytesGT h1 e) (Plain.plain_to_bytesGT h1 sh)
+                /\ modifies_none h0 h1
+              ))
+            ) ->
+            om_base_point: lbytes om_dh_share_length ->
+            om_im:ID.index_module{ID.id om_im == lbytes om_dh_share_length} ->
+            om_kim:ID.index_module{ID.id om_kim == i:(plain_bytes om_spm * plain_bytes om_spm){b2t (smaller' om_dh_share_length (fst i) (snd i))}} ->
+            om_km:Key.key_module om_kim{Key.get_keylen om_km = om_hash_length /\ Key.get_pm om_km == om_kpm} ->
             om_rgn:Key.log_region ->
             om:odh_module{
               om.kim == om_kim /\
-              (let om_km:(km:Key.key_module om.kim{Key.get_keylen om.kim km = om_hash_len}) = om_km in
-              get_hash_length om = om_hash_len
-              /\ get_dh_share_length om = om_dh_share_len
-              /\ get_dh_exponent_length om = om_dh_exponent_len
+              (let om_km:(km:Key.key_module om.kim{Key.get_keylen km = om_hash_length}) = om_km in
+              get_hash_length om = om_hash_length
+              /\ om_kpm == om.kpm
+              /\ om_epm == om.epm
+              /\ om_spm == om.spm
+              /\ get_dh_share_length om = om_dh_share_length
+              /\ get_dh_exponent_length om = om_dh_exponent_length
               /\ get_index_module om == om_im
               /\ get_key_index_module om == om_kim
-              /\ (let km:(k:Key.key_module om_kim{Key.get_keylen om_kim k = om_hash_len}) = om_km in
-                let fun_km:(k:Key.key_module om_kim{Key.get_keylen om_kim k = om_hash_len}) = get_key_module om om_kim in
+              /\ (let km:(k:Key.key_module om_kim{Key.get_keylen k = om_hash_length}) = om_km in
+                let fun_km:(k:Key.key_module om_kim{Key.get_keylen k = om_hash_length}) = get_key_module om om_kim in
               fun_km == km)
-              /\ hash_fun om == om_hash_fun
-              /\ dh_exponentiate om == om_exponentiate
-              /\ get_base_point om == om_base_point)
+              /\ hash_fun #om == om_hash_low
+              /\ dh_exponentiate #om == om_exponentiate_low
+              /\ om_base_point == om.base_point
+              )
             }
 
 (**
@@ -105,69 +181,83 @@ val create: om_hash_len:nat ->
 //val skey: om:odh_module -> skey'
 
 
+val pk_get_share_bytesGT: (#om:odh_module) -> (pk:pkey om) -> (sh:dh_share_bytes om)
 
 (**
   A helper function to obtain the raw bytes of a DH public key.
 *)
-val pk_get_share: om:odh_module -> pk:pkey om -> Tot (dh_sh:dh_share om) //{dh_sh = pk.pk_share})
+val pk_get_share: #om:odh_module -> pk:pkey om -> StackInline (dh_sh:dh_share om) //{dh_sh = pk.pk_share})
+  (requires (fun h ->
+    0 < normalize_term (Seq.length (pk_get_share_bytesGT pk))
+    /\ normalize_term (Seq.length (pk_get_share_bytesGT pk)) <= UInt.max_int 32
+  ))
+  (ensures (fun (h0:mem) p h1 ->
+     let len = Plain.plain_length p in
+     len > 0
+     /\ ~(Buffer.contains h0 p)
+     /\ Buffer.live h1 p /\ Buffer.idx p = 0 /\ Plain.plain_length p = len
+     /\ Buffer.frameOf p = h0.tip
+     /\ Map.domain h1.h == Map.domain h0.h
+     /\ Buffer.modifies_0 h0 h1
+     /\ Plain.plain_to_bytesGT h1 p == pk_get_share_bytesGT pk
+   ))
 
-val lemma_pk_get_share_inj: om:odh_module -> pk:pkey om -> Lemma
-  (requires True)
-  (ensures (forall pk' . pk_get_share om pk' == pk_get_share om pk <==> pk' == pk))
-  [SMTPat (pk_get_share om pk)]
 
-val get_skeyGT: om:odh_module -> sk:skey om -> GTot (raw:dh_exponent om) //{raw=sk.sk_exp})
+val get_skeyGT: #om:odh_module -> sk:skey om -> GTot (raw:dh_exponent_bytes om) //{raw=sk.sk_exp})
 
 #set-options "--z3rlimit 300 --max_ifuel 1 --max_fuel 0"
 (**
 A helper function to obtain the share that corresponds to a DH secret key.
 *)
-val sk_get_share: om:odh_module -> sk:skey om -> Tot (dh_sh:dh_share om{dh_sh = share_from_exponent om (get_skeyGT om sk)})
+val sk_get_share_bytesGT: #om:odh_module -> sk:skey om -> GTot (dh_sh:dh_share_bytes om)
+val sk_get_share: (#om:odh_module) -> (sk:skey om) -> StackInline (dh_sh:dh_share om)
+  (requires (fun h ->
+    0 < normalize_term (Seq.length (sk_get_share_bytesGT sk))
+    /\ normalize_term (Seq.length (sk_get_share_bytesGT sk)) <= UInt.max_int 32
+  ))
+  (ensures (fun (h0:mem) p h1 ->
+     let len = Plain.plain_length p in
+     len > 0
+     /\ ~(Buffer.contains h0 p)
+     /\ Buffer.live h1 p /\ Buffer.idx p = 0 /\ Plain.plain_length p = len
+     /\ Buffer.frameOf p = h0.tip
+     /\ Map.domain h1.h == Map.domain h0.h
+     /\ Buffer.modifies_0 h0 h1
+     /\ Plain.plain_to_bytesGT h1 p == sk_get_share_bytesGT sk
+   ))
 
-val leak_skey: om:odh_module -> sk:skey om{ID.dishonest om.im (sk_get_share om sk)} -> Tot (raw:dh_exponent om{raw=get_skeyGT om sk})
+val compatible_keys: #om:odh_module -> sk:skey om -> pk:pkey om -> t:Type0{t <==> pk_get_share_bytesGT pk =!= sk_get_share_bytesGT sk}
 
-val keygen: om:odh_module -> ST (dh_pair:(pkey om * skey om){fst dh_pair == get_pkey om (snd dh_pair)})
+val leak_skey: #om:odh_module -> sk:skey om{ID.dishonest om.im (sk_get_share_bytesGT sk) \/ ~Flags.prf_odh} -> Tot (raw:dh_exponent_bytes om{raw=get_skeyGT sk})
+
+val keygen: #om:odh_module -> ST (dh_pair:(pkey om * skey om))
   (requires (fun h0 -> True))
-  (ensures (fun h0 _ h1 -> modifies_none h0 h1))
+  (ensures (fun h0 dh_pair h1 ->
+    modifies_none h0 h1
+    /\ fst dh_pair == get_pkey (snd dh_pair)
+  ))
 
-val coerce_pkey: om:odh_module -> dh_sh:dh_share om{ID.dishonest om.im dh_sh} -> Tot (pk:pkey om{pk_get_share om pk=dh_sh})
+val coerce_pkey: #om:odh_module -> dh_sh:dh_share_bytes om{ID.dishonest om.im (dh_sh) \/ ~Flags.prf_odh} -> (pkey om)
 
 (**
   coerce_keypair allows the adversary to coerce a DH exponent into a DH private key. The corresponding DH public key
   is generated along with it. Both keys are considered dishonest and the id is considered unfresh after coercion.
 *)
-val coerce_keypair: om:odh_module -> dh_exp:dh_exponent om{ID.dishonest om.im (share_from_exponent om dh_exp)} -> Tot (dh_pair:(k:pkey om{pk_get_share om k = share_from_exponent om dh_exp}) * (k:skey om{get_skeyGT om k=dh_exp}))
+val coerce_keypair: #om:odh_module -> dh_exp:dh_exponent_bytes om{ID.dishonest om.im (om.exponentiate dh_exp om.base_point)} -> ((pkey om) * (skey om))
 
-
-val compose_ids: om:odh_module -> s1:dh_share om -> s2:dh_share om{s2 <> s1} -> (i:(dh_share om * dh_share om){b2t (smaller om (fst i) (snd i))})
+val compose_ids: om:odh_module -> s1:dh_share_bytes om -> s2:dh_share_bytes om{s2 <> s1} -> (i:(dh_share_bytes om * dh_share_bytes om){b2t (smaller om (fst i) (snd i))})
 
 (**
   GTot specification of the prf_odh function for use in type refinements.
 *)
-val prf_odhGT: om:odh_module -> sk:skey om -> pk:pkey om{compatible_keys om sk pk} -> GTot (ho:hash_output om{ho = hash_fun om (dh_exponentiate om (get_skeyGT om sk) (pk_get_share om pk))})
+val prf_odhGT: #om:odh_module -> sk:skey om -> pk:pkey om{compatible_keys sk pk} -> GTot (ho:hash_output_bytes om{ho == om.hash (om.exponentiate (get_skeyGT sk) (pk_get_share_bytesGT pk))})
 
-val lemma_shares: om:odh_module -> sk:skey om -> Lemma
-  (requires True)
-  (ensures (pk_get_share om (get_pkey om sk)) == sk_get_share om sk)
-  [ SMTPat (sk_get_share om sk)]
-
-#set-options "--z3rlimit 1000 --max_ifuel 1 --max_fuel 0"
-val prf_odh: om:odh_module -> sk:skey om -> pk:pkey om{compatible_keys om sk pk} -> ST (k:Key.get_keytype om.kim om.km)
-  (requires (fun h0 ->
-    let i = compose_ids om (pk_get_share om pk) (sk_get_share om sk) in
-    ID.registered om.kim i
-    /\ Key.invariant om.kim om.km h0
-  ))
-  (ensures (fun h0 k h1 ->
-    let i = compose_ids om (pk_get_share om pk) (sk_get_share om sk) in True
-    /\ Key.get_index om.kim om.km k = i
-    /\ ((ID.honest om.kim i /\ b2t Flags.prf_odh) ==>
-        modifies (Set.singleton (Key.get_log_region om.kim om.km)) h0 h1)
-    // We should guarantee, that the key is randomly generated. Generally, calls to prf_odh should be idempotent. How to specify that?
-    // Should we have a genPost condition that we guarantee here?
-    /\ ((ID.dishonest om.kim i \/ ~(b2t Flags.prf_odh)) ==>
-        (Key.get_rawGT om.kim om.km k = prf_odhGT om sk pk // Functional correctness.
-        /\ h0 == h1))
-    /\ (modifies (Set.singleton (Key.get_log_region om.kim om.km))h0 h1 \/ h0 == h1)
-    /\ Key.invariant om.kim om.km h1
-  ))
+//val lemma_shares: om:odh_module -> sk:skey om -> Lemma
+//  (requires True)
+//  (ensures (pk_get_share om (get_pkey om sk)) == sk_get_share om sk)
+//  [ SMTPat (sk_get_share om sk)]
+//
+//val lemma_share_bytes: om:odh_module -> sk:skey om -> Lemma
+//  (requires True)
+//  (ensures (pk_get_share_bytesGT om (get_pkey om sk)) == sk_get_share_bytesGT om sk)
+//  [ SMTPat (sk_get_share_bytesGT om sk)]
