secure_api/box/Box.PKAE.fst
@@ -3,7 +3,6 @@
 *)
 module Box.PKAE
 
-
 open FStar.Set
 open FStar.HyperHeap
 open FStar.HyperStack
@@ -32,85 +31,148 @@ module AE = Box.AE
 module LE = FStar.Endianness
 
 #set-options "--z3rlimit 600 --max_ifuel 1 --max_fuel 0"
-let nonce = AE.nonce
-let cipher = AE.cipher
-let sub_id  = lbytes Curve.serialized_point_length
-let key_id = (i:(lbytes Curve.serialized_point_length*lbytes Curve.serialized_point_length){b2t (ODH.smaller' Curve.serialized_point_length (fst i) (snd i))})
-let plain = AE.ae_plain
+//let nonce = AE.nonce
+//let cipher = AE.cipher
+//let sub_id  = lbytes Curve.serialized_point_length
+//let key_id = (i:(lbytes Curve.serialized_point_length*lbytes Curve.serialized_point_length){b2t (ODH.smaller' Curve.serialized_point_length (fst i) (snd i))})
+//let plain = AE.ae_plain
 
 
-let valid_plain_length = AE.valid_plain_length
-let valid_cipher_length = AE.valid_cipher_length
+//let valid_plain_length = AE.valid_plain_length
+//let valid_cipher_length = AE.valid_cipher_length
 
 let zero_nonce = Seq.create HSalsa.noncelen (UInt8.uint_to_t 0)
 let hsalsa20_hash input = HSalsa.hsalsa20 input zero_nonce
 
 let base_point:lbytes Curve.serialized_point_length = Curve.base_point
 
+let pkey_len = Curve.serialized_point_length
+let skey_len = Curve.scalar_length
+let sub_id = b:bytes{Seq.length b = Curve.serialized_point_length}
+let key_id = i:(sub_id * sub_id){b2t (ODH.smaller' Curve.serialized_point_length (fst i) (snd i))}
+
+let valid_plain_length n = n / Spec.Salsa20.blocklen < pow2 32
+let plain_buffer = b:FStar.Buffer.buffer UInt8.t{valid_plain_length (FStar.Buffer.length #UInt8.t b)}
+
+
+val buffer_length_lemma: unit -> Lemma
+  (requires True)
+  (ensures forall (b:plain_buffer) . valid_plain_length (FStar.Buffer.length b))
+let buffer_length_lemma() = ()
+
+let buffer_to_bytesST n b = FStar.Buffer.to_seq #plain_buffer b n
+let bytes_to_bufferST n b = FStar.Buffer.create b n
+let buffer_to_bytesGT n b = FStar.Buffer.as_seq
+
+let ppm = Plain.create (FStar.Buffer.buffer UInt8.t)
+                       (fun n -> n / Spec.Salsa20.blocklen < pow2 32)
+                       (FStar.Buffer.length)
+                       (buffer_length_lemma)
+                       (FStar.Buffer.as_seq)
+                       (buffer_to_bytesST)
+                       (bytes_to_bufferST)
+
+
+val cpm:wire_module
+val pkpm:wire_module
+val skpm:wire_module
+val npm:wire_module
 #set-options "--z3rlimit 600 --max_ifuel 1 --max_fuel 0"
-private noeq type aux_t' (im:index_module) (kim:plain_index_module) (pm:Plain.plain_module) (rgn:log_region) =
+private noeq type aux_t'
+                         (im:ID.index_module)
+                         (kim:ID.index_module)
+                         (rgn:log_region)
+                         =
   | AUX:
-    am:AE.ae_module kim{extends (AE.get_message_log_region #kim am) rgn /\ AE.get_pm am == pm} ->
+    am:AE.ae_module kim{extends (AE.get_message_log_region #kim am) rgn
+                        /\ AE.get_ppm am == ppm
+                        /\ AE.get_cpm am == cpm
+                        /\ AE.get_npm am == npm} ->
     om:ODH.odh_module{ODH.get_hash_length om = HSalsa.keylen
                       /\ ODH.get_dh_share_length om = Curve.serialized_point_length
                       /\ ODH.get_dh_exponent_length om = Curve.scalar_length
-                      /\ ODH.dh_exponentiate om == Curve.scalarmult
-                      /\ ODH.hash_fun om == hsalsa20_hash
-                      /\ ODH.get_base_point om = base_point
+                      ///\ ODH.dh_exponentiate om == Curve.scalarmult
+                      ///\ ODH.hash_fun om == hsalsa20_hash
+                      ///\ ODH.get_base_point om = base_point
                       /\ ODH.get_index_module om == im
                       /\ ODH.get_key_index_module om == kim
+                      /\ ODH.get_kpm om == AE.get_kpm am
+                      /\ ODH.get_spm om == pkpm
+                      /\ ODH.get_epm om == skpm
                       } ->
     km:Key.key_module kim{
                           km == ODH.get_key_module om kim
                           /\ km == AE.instantiate_km am
-                          /\ Key.get_keylen kim km == ODH.get_hash_length om
-                          /\ extends (Key.get_log_region kim km) rgn} ->
-    aux_t' im kim pm rgn
+                          /\ Key.get_keylen km == ODH.get_hash_length om
+                          /\ extends (Key.get_log_region km) rgn} ->
+    aux_t' im kim ppm cpm pkpm skpm npm rgn
 
-let aux_t im kim pm rgn = aux_t' im kim pm rgn
+let aux_t im kim ppm cpm pkpm skpm npm rgn = aux_t' im kim ppm cpm pkpm skpm npm rgn
+
+let compute_cipher_length pkm = AE.compute_cipher_length pkm.aux.am
+let compute_plain_length pkm = AE.compute_plain_length pkm.aux.am
+
+val enc: pkm:pkae_module -> (p:wire_bytes #pkm.ppm -> wire_bytes #pkm.npm -> wire_bytes #pkm.pkpm -> wire_bytes #pkm.skpm -> Tot (c:bytes{Seq.length c = compute_cipher_length pkm (Seq.length p)}))
+val dec: pkm:pkae_module -> (c:wire_bytes #pkm.cpm -> wire_bytes #pkm.npm -> wire_bytes #pkm.pkpm -> wire_bytes #pkm.skpm -> Tot (option (p:bytes{Seq.length p = compute_plain_length pkm (Seq.length c)})))
+let enc pkm = SPEC.cryptobox
+let dec pkm = SPEC.cryptobox_open
 
 let skey pkm = ODH.skey pkm.aux.om
 let pkey pkm = ODH.pkey pkm.aux.om
 
+#set-options "--z3rlimit 600 --max_ifuel 1 --max_fuel 0"
 let pkey_from_skey pkm sk = ODH.get_pkey pkm.aux.om sk
+let pkey_raw_from_skey pkm sk = ODH.sk_get_share_bytesGT pkm.aux.om sk
+let pkey_get_raw pkm pk = ODH.pk_get_share pkm.aux.om pk
+let skey_get_raw pkm sk = ODH.get_skeyGT pkm.aux.om sk
+
+let pkey_to_subId #pkm pk = ODH.pk_get_share pkm.aux.om pk
+//let pkey_to_subId_inj #pkm pk = ODH.lemma_pk_get_share_inj pkm.aux.om pk
+
+
 let compatible_keys pkm sk pk = ODH.compatible_keys pkm.aux.om sk pk
 
-let enc pkm p n pk sk =
-  SPEC.cryptobox p n (ODH.pk_get_share pkm.aux.om pk) (ODH.get_skeyGT pkm.aux.om sk)
-
-let dec pkm c n pk sk =
-  let p = SPEC.cryptobox_open c n (ODH.pk_get_share pkm.aux.om pk) (ODH.get_skeyGT pkm.aux.om sk) in
-  match p with
-  | Some p' ->
-    let p'':plain = p' in
-    Some p''
-  | None -> None
+//let enc pkm p n pk sk =
+//  SPEC.cryptobox p n (ODH.pk_get_share pkm.aux.om pk) (ODH.get_skeyGT pkm.aux.om sk)
+//
+//let dec pkm c n pk sk =
+//  let p = SPEC.cryptobox_open c n (ODH.pk_get_share pkm.aux.om pk) (ODH.get_skeyGT pkm.aux.om sk) in
+//  match p with
+//  | Some p' ->
+//    let p'':plain = p' in
+//    Some p''
+//  | None -> None
 
 #set-options "--z3rlimit 600 --max_ifuel 1 --max_fuel 1"
 let compose_ids pkm i1 i2 = ODH.compose_ids pkm.aux.om i1 i2
 
-let length pkm = AE.length
+//let key_index_module = plain_index_module
+//let plain_module = pm:Plain.plain_module{Plain.get_plain pm == plain /\ Plain.valid_length #pm == valid_plain_length}
 
-
-let key_index_module = plain_index_module
-let plain_module = pm:Plain.plain_module{Plain.get_plain pm == plain /\ Plain.valid_length #pm == valid_plain_length}
-
-#set-options "--z3rlimit 600 --max_ifuel 1 --max_fuel 1"
-val message_log_lemma: im:key_index_module -> rgn:log_region{disjoint (ID.get_rgn im) rgn} -> Lemma
+#set-options "--z3rlimit 1600 --max_ifuel 2 --max_fuel 0 --__temp_no_proj Box.PKAE"
+val message_log_lemma: pkm:pkae_module -> rgn:log_region{disjoint (ID.get_rgn pkm.pim) rgn} -> Lemma
   (requires True)
-  (ensures message_log im rgn === AE.message_log im rgn)
-let message_log_lemma im rgn =
-  assert(FStar.FunctionalExtensionality.feq (message_log_value im) (AE.message_log_value im));
-  assert(FStar.FunctionalExtensionality.feq (message_log_range im) (AE.message_log_range im));
-  let inv = message_log_inv im in
-  let map_t =MM.map' (message_log_key im) (message_log_range im) in
+  (ensures message_log pkm.pim pkm.cpm pkm.ppm pkm.npm rgn === AE.message_log pkm.pim pkm.cpm pkm.ppm pkm.npm rgn)
+let message_log_lemma pkm rgn =
+  //assume(AE.ae_plain == plain pkm);
+  //assume(AE.cipher == cipher pkm);
+  //assume(AE.nonce == nonce pkm);
+  //assume(pkm.key_id == ID.id pkm.pim);
+  assert((message_log_key pkm.pim pkm.npm) == (AE.message_log_key pkm.pim pkm.npm));
+  let ae_efun:((message_log_key pkm.pim pkm.npm) -> Type0) = AE.message_log_range pkm.pim pkm.ppm pkm.cpm pkm.npm in
+  //admit();
+  assert(FStar.FunctionalExtensionality.feq (message_log_value pkm.pim) (AE.message_log_value pkm.pim));
+  assert(FStar.FunctionalExtensionality.feq (message_log_range pkm.pim pkm.ppm pkm.cpm pkm.npm) (AE.message_log_range pkm.pim pkm.ppm pkm.cpm pkm.npm));
+  //admit();
+  let inv = message_log_inv pkm.pim pkm.cpm pkm.ppm pkm.npm in
+  let map_t =MM.map' (message_log_key pkm.pim pkm.npm) (message_log_range pkm.pim pkm.ppm pkm.cpm pkm.npm) in
   let inv_t = map_t -> Type0 in
-  let ae_inv = AE.message_log_inv im in
+  let ae_inv = AE.message_log_inv pkm.pim pkm.ppm pkm.cpm pkm.npm in
   let ae_inv:map_t -> Type0 = ae_inv in
   assert(FStar.FunctionalExtensionality.feq
     #map_t #Type
     inv ae_inv);
-  assert(message_log im rgn == AE.message_log im rgn);
+  assert(message_log pkm.pim pkm.ppm pkm.cpm pkm.npm rgn == AE.message_log pkm.pim pkm.ppm pkm.cpm pkm.npm rgn);
   ()
 
 
@@ -169,9 +231,6 @@ let key (pkm:pkae_module) = AE.key pkm.pim
 
 let zero_bytes = AE.create_zero_bytes
 
-let pkey_to_subId #pkm pk = ODH.pk_get_share pkm.aux.om pk
-let pkey_to_subId_inj #pkm pk = ODH.lemma_pk_get_share_inj pkm.aux.om pk
-
 let nonce_is_fresh (pkm:pkae_module) (i:ID.id pkm.pim) (n:nonce) (h:mem) =
   AE.nonce_is_fresh pkm.aux.am i n h
 
@@ -220,27 +279,32 @@ let buf_to_seq (b:uint8_p): Stack (seq FStar.UInt8.t) (requires (fun h -> live h
 let as_seq h (b:uint8_p) =
   seq_of_list (FStar.List.Tot.map declassify_u8 (seq_to_list (Buffer.as_seq h b)))
 
-let seq_to_buf (b:uint8_p) (s:seq FStar.UInt8.t): unit =
-  admit()
+assume val seq_to_buf: (s:seq FStar.UInt8.t) -> St (b:uint8_p)
 
 let pkm = my_create root
 
+#set-options "--z3rlimit 1000 --max_ifuel 1 --max_fuel 0"
+val transmute_bytes_to_buffer: #pkm:pkae_module -> #i:ID.id pkm.pim -> p1:Plain.protected_plain_t pkm.pim plain i -> St (p2:Plain.protected_plain_t pkm.pim (Buffer.buffer Hacl.UInt8.t) i)
+let transmute_bytes_to_buffer #pkm #i p1 =
+  Plain.transmute_protected_plainST #pkm.pim #i #plain #uint8_p seq_to_buf p1
+
 val encrypt_low:
   pkm:pkae_module ->
-  c:uint8_p ->
-  m:uint8_p -> //we might want this to be abstract
-  mlen:u64{let len = U64.v mlen in length c = len /\ len = length m}  ->
-  n:uint8_p ->
   sk:skey pkm -> //I use the abstract high level keys here
   pk:pkey pkm ->
+  c:uint8_p ->
+  m:Plain.protected_plain_t pkm.pim uint8_p (compose_ids pkm (pkey_to_subId #pkm pk) (pkey_to_subId #pkm (pkey_from_skey pkm sk))) ->
+  mlen:u64{let len = U64.v mlen in length c = len /\ len = Plain.length #pkm.pim #pkm.pm m}  ->
+  n:uint8_p ->
   Stack u32
-    (requires (fun h -> live h c /\ live h m /\ live h n))  //we have to add the security specification here
+    (requires (fun h -> live h c /\ Plain.live m h /\ live h n))  //we have to add the security specification here
     (ensures  (fun h0 z h1 -> modifies_1 c h0 h1 /\ live h1 c /\
       ( let r = as_seq h1 c in
-        let m = as_seq h1 m in
+        let m = as_seq h1 (Plain.make_plainGT #pkm.im #pkm.pm m) in
         r = SPEC.cryptobox m (as_seq h1 n) (ODH.pk_get_share pkm.aux.om pk) (ODH.get_skeyGT pkm.aux.om sk) )))
-let encrypt_low c m mlen n sk pk =
-  let m = buf_to_seq m in
+let encrypt_low pkm sk pk c m mlen n =
+  let i = compose_ids pkm (pkey_to_subId #pkm pk) (pkey_to_subId #pkm (pkey_from_skey pkm sk)) in
+  let m = Plain.transmute_protected_plainST #pkm.im #i #uint8_p #plain buf_to_seq m in
   let n = buf_to_seq n in
   let m = admit() in //conversion from m to abstract plaintext?
   let c' = encrypt pkm n sk pk m in
