secure_api/box/Box.PKAE.fsti
@@ -22,65 +22,71 @@ module Plain = Box.Plain
 module ID = Box.Index
 
 
-val nonce: t:Type0{hasEq t}
-val cipher: Type0
-val sub_id: t:Type0{hasEq t}
-val key_id: Type0
-val plain: Type0
-
-val valid_plain_length: nat -> bool
-val valid_cipher_length: nat -> bool
-
-let index_module = im:ID.index_module{ID.id im == sub_id}
-let plain_index_module = im:ID.index_module{ID.id im == key_id}
+//let index_module = im:ID.index_module{ID.id im == sub_id}
+//let plain_index_module = im:ID.index_module{ID.id im == key_id}
 
 let log_region =
   r:MR.rid{is_eternal_region r}
 
-val aux_t: (im:index_module) -> (kim:plain_index_module) -> (pm:Plain.plain_module) -> (rgn:log_region) -> Type u#1
 
+let wire_module = Plain.wire_module
+let index_module = ID.index_module
+let id = ID.id
+let wire (pm:wire_module) = Plain.get_wire_t pm
+let protected_plain (#im:index_module) (#pm:wire_module) (i:id im) = p:Plain.protected_wire_t im (pt:Plain.get_wire_t pm) i{Plain. valid_wire_length pm (Plain.make_wire_tGT p)}
+let wire_bytes (#pm:wire_module) = b:bytes{Plain.valid_length pm (Seq.length b)}
+
+
+val pkey_len: nat
+val skey_len: nat
+val sub_id:eqtype
+val key_id: Type0
+
+let im = (im:ID.index_module{ID.id im == sub_id})
+let pim = (pim:ID.index_module{ID.id pim == key_id})
+
+
+val ppm:wire_module
+val cpm:wire_module
+val pkpm:wire_module
+val skpm:wire_module
+val npm:wire_module
+
+val aux_t: (im:ID.index_module) -> (kim:ID.index_module) -> (rgn:log_region) -> Type u#1
+
+#set-options "--__temp_no_proj Box.PKAE"
 abstract noeq type pkae_module =
   | PKAE:
     im:ID.index_module{ID.id im == sub_id} ->
     pim:ID.index_module{ID.id pim == key_id} ->
-    pm:Plain.plain_module{Plain.get_plain pm == plain /\ Plain.valid_length #pm == valid_plain_length} ->
+    ppm:Plain.wire_module ->
+    cpm:wire_module ->
+    pkpm:wire_module{Plain.valid_length pkpm == (fun n -> n = pkey_len)} ->
+    skpm:wire_module{Plain.valid_length skpm == (fun n -> n = skey_len)} ->
+    npm:wire_module ->
     rgn:log_region ->
-//    enc: (plain -> n:nonce -> pk:pkey -> sk:skey{compatible_keys sk pk} -> GTot cipher) ->
-//    dec: (c:cipher -> n:nonce -> pk:pkey -> sk:skey{compatible_keys sk pk} -> GTot (option plain)) ->
-    aux: aux_t im pim pm rgn ->
+    aux: aux_t im pim rgn ->
     pkae_module
 
+val compute_cipher_length: (pkm:pkae_module) -> (plain_len:nat{Plain.valid_length pkm.ppm plain_len} -> cipher_len:nat{Plain.valid_length pkm.cpm cipher_len})
+val compute_plain_length:  (pkm:pkae_module) -> (cipher_len:nat{Plain.valid_length pkm.cpm cipher_len} -> plain_len:nat{Plain.valid_length pkm.ppm plain_len})
+
+//val enc: pkm:pkae_module -> (p:wire_bytes #pkm.ppm -> wire_bytes #pkm.npm -> wire_bytes #pkm.pkpm -> wire_bytes #pkm.skpm -> Tot (c:bytes{Seq.length c = compute_cipher_length pkm (Seq.length p)}))
+//val dec: pkm:pkae_module -> (c:wire_bytes #pkm.cpm -> wire_bytes #pkm.npm -> wire_bytes #pkm.pkpm -> wire_bytes #pkm.skpm -> Tot (option (p:bytes{Seq.length p = compute_plain_length pkm (Seq.length c)})))
+
+#reset-options
 val skey: pkae_module -> Type0
 val pkey: pkae_module -> Type0
 
 val pkey_from_skey: (pkm:pkae_module -> sk:skey pkm -> pk:pkey pkm)
+val pkey_get_raw: (pkm:pkae_module) -> (pkey pkm) -> wire pkm.pkpm
+val skey_get_raw: (pkm:pkae_module) -> (skey pkm) -> GTot (wire_bytes #pkm.skpm)
 
-val compatible_keys: (pkm:pkae_module -> sk:skey pkm -> pk:pkey pkm -> t:Type0{t <==> pk =!= pkey_from_skey pkm sk})
+let pkey_get_raw_bytesGT (pkm:pkae_module) (pk:pkey pkm) = Plain.wire_t_to_bytesGT pkm.pkpm (pkey_get_raw pkm pk)
 
-val enc (pkm:pkae_module): plain -> n:nonce -> pk:pkey pkm -> sk:skey pkm{compatible_keys pkm sk pk} -> GTot cipher
-val dec (pkm:pkae_module): c:cipher -> n:nonce -> pk:pkey pkm -> sk:skey pkm{compatible_keys pkm sk pk} -> GTot (option plain)
-
-val compose_ids: pkae:pkae_module ->  s1:sub_id -> s2:sub_id{s2 <> s1} -> key_id
-
-val length: pkae:pkae_module -> p:plain -> n:nat{valid_plain_length n}
-
-
-
-type message_log_key (im:plain_index_module) = (nonce*(i:ID.id im))
-type message_log_value (im:plain_index_module) (i:ID.id im) = (cipher*Plain.protected_plain_t im plain i)
-type message_log_range (im:plain_index_module) (k:message_log_key im) = (v:message_log_value im (snd k))
-type message_log_inv (im:plain_index_module) (f:MM.map' (message_log_key im) (message_log_range im)) = True //t:Type0{t = True}
-type message_log (im:plain_index_module) (rgn:log_region) =
-  MM.t rgn (message_log_key im) (message_log_range im) (message_log_inv im)
-
-
-val get_message_log_region: pkm:pkae_module -> Tot (lr:log_region{extends lr pkm.rgn})
-val get_message_logGT: pkm:pkae_module -> Tot (message_log pkm.pim (get_message_log_region pkm)) //TODO: MK: would prefer this to be GTot
-
-val create: rgn:rid -> St (pkm:pkae_module)
-
-val zero_bytes: (n:nat{valid_plain_length n}) -> plain //b:bytes{Seq.length b = n /\ b=Seq.create n (UInt8.uint_to_t 0)}
-//TODO: MK this can be modelled better
+let cipher (pkm:pkae_module) = (c:Plain.get_wire_t pkm.cpm)
+let plain (pkm:pkae_module) = (p:Plain.get_wire_t pkm.ppm)
+let nonce (pkm:pkae_module) = (n:Plain.get_wire_t pkm.npm )
 
 val pkey_to_subId: #pkm:pkae_module -> pk:pkey pkm -> ID.id pkm.im
 val pkey_to_subId_inj: #pkm:pkae_module -> pk:pkey pkm -> Lemma
@@ -88,16 +94,40 @@ val pkey_to_subId_inj: #pkm:pkae_module -> pk:pkey pkm -> Lemma
   (ensures (forall pk' . pkey_to_subId #pkm pk == pkey_to_subId #pkm pk' <==> pk == pk'))
   [SMTPat (pkey_to_subId #pkm pk)]
 
+val compatible_keys: (pkm:pkae_module -> sk:skey pkm -> pk:pkey pkm -> t:Type0{t <==> (pkey_to_subId pk) =!= pkey_to_subId (pkey_from_skey pkm sk)})
+
+//val enc (pkm:pkae_module): plain pkm -> n:nonce pkm -> pk:pkey pkm -> sk:skey pkm{compatible_keys pkm sk pk} -> GTot (cipher pkm)
+//val dec (pkm:pkae_module): c:cipher pkm -> n:nonce pkm -> pk:pkey pkm -> sk:skey pkm{compatible_keys pkm sk pk} -> GTot (option (plain pkm))
+
+val compose_ids: pkm:pkae_module ->  s1:sub_id -> s2:sub_id{s2 <> s1} -> key_id
+
+//val length: pkae:pkae_module -> p:plain -> n:nat{valid_plain_length n}
+
+
+
+// Message log types
+let message_log_key (im:index_module) (npm:wire_module) = (wire_bytes #npm*(i:id im))
+let message_log_value (im:index_module) (cpm:wire_module) (ppm:wire_module) (i:id im) = (c:wire_bytes #cpm*m:protected_plain #im #ppm i)
+let message_log_range (im:index_module) (cpm:wire_module) (ppm:wire_module) (npm:wire_module) (k:message_log_key im npm) = (message_log_value im cpm ppm (snd k))
+let message_log_inv (im:index_module) (cpm:wire_module) (ppm:wire_module) (npm:wire_module) (f:MM.map' (message_log_key im npm) (message_log_range im cpm ppm npm)) = True
+
+let message_log (im:index_module) (cpm:wire_module) (ppm:wire_module) (npm:wire_module) (rgn:log_region) =
+  MM.t rgn (message_log_key im npm) (message_log_range im cpm ppm npm) (message_log_inv im cpm ppm npm)
+
+
+val get_message_log_region: pkm:pkae_module -> Tot (lr:log_region{extends lr pkm.rgn})
+val get_message_logGT: pkm:pkae_module -> Tot (message_log pkm.pim pkm.cpm pkm.ppm pkm.npm (get_message_log_region pkm)) //TODO: MK: would prefer this to be GTot
+
+val create: rgn:rid -> St (pkm:pkae_module)
+
+val zero_bytes: n:nat -> Tot (b:bytes{b=Seq.create n (UInt8.uint_to_t 0)})
+//TODO: MK this can be modelled better
+
 #set-options "--z3rlimit 2000 --max_ifuel 1 --max_fuel 0"
-val nonce_is_fresh: (pkm:pkae_module) -> (i:ID.id pkm.pim) -> (n:nonce) -> (h:mem) ->
+val nonce_is_fresh: (pkm:pkae_module) -> (i:ID.id pkm.pim) -> (n:nonce pkm) -> (h:mem) ->
   (t:Type0{t <==>
-    (MR.m_contains #(get_message_log_region pkm) (get_message_logGT pkm) h
-      /\ MM.fresh #(get_message_log_region pkm)(get_message_logGT pkm) (n,i) h)})
-
-
-//val pkey_from_skey_inj: sk:skey -> pk:pkey -> Lemma
-//  (requires True)
-//  (ensures (forall sk1 sk2 . pkey_from_skey sk1 == pkey_from_skey sk2 <==> sk1 == sk2))
+    (MR.m_contains (get_message_logGT pkm) h
+    /\ MM.fresh (get_message_logGT pkm) ((Plain.wire_t_to_bytesGT pkm.npm n),i) h)})
 
 val invariant: pkae_module -> mem -> Type0
 
@@ -112,11 +142,11 @@ let honest pkm i = ID.honest pkm.pim i
 let dishonest pkm i = ID.dishonest pkm.pim i
 
 val encrypt: pkm:pkae_module ->
-             n:nonce ->
+             n:nonce pkm ->
              sk:skey pkm ->
              pk:pkey pkm{compatible_keys pkm sk pk} ->
-             m:(Plain.protected_plain_t pkm.pim (Plain.get_plain pkm.pm) (compose_ids pkm (pkey_to_subId #pkm pk) (pkey_to_subId #pkm (pkey_from_skey pkm sk)))) ->
-             ST cipher
+             p:(protected_plain #pkm.pim #pkm.ppm (compose_ids pkm (pkey_to_subId #pkm pk) (pkey_to_subId #pkm (pkey_from_skey pkm sk)))) ->
+             ST (cipher pkm)
   (requires (fun h0 ->
     let i = compose_ids pkm (pkey_to_subId #pkm pk) (pkey_to_subId #pkm (pkey_from_skey pkm sk)) in
     registered pkm i
@@ -127,23 +157,24 @@ val encrypt: pkm:pkae_module ->
   (ensures  (fun h0 c h1 ->
     let i = compose_ids pkm (pkey_to_subId #pkm pk) (pkey_to_subId #pkm (pkey_from_skey pkm sk)) in
     True //modifies (Set.singleton pkm.rgn) h0 h1 // stateful changes even if the id is dishonest.
-    /\ ((honest pkm i /\ b2t pkae) // Ideal behaviour if the id is honest and the assumption holds
-               ==> eq2 #cipher c (enc pkm (zero_bytes (Plain.length #pkm.pim #pkm.pm #i m)) n pk sk))
-    /\ ((dishonest pkm i \/ ~(b2t pkae)) // Concrete behaviour otherwise.
-                  ==> eq2 #cipher c (enc pkm (Plain.repr #pkm.pim #pkm.pm #i m) n pk sk))
+    /\ ((honest pkm i /\ b2t ae_ind_cpa) // Ideal behaviour if the id is honest and the assumption holds.
+      ==> ((Plain.wire_t_to_bytesGT pkm.cpm c) == enc pkm (zero_bytes (Plain.length #pkm.pim #pkm.ppm #(compose_ids pkm (pkey_to_subId #pkm pk) (pkey_to_subId #pkm (pkey_from_skey pkm sk))) p)) (Plain.wire_t_to_bytesGT pkm.pkpm (pkey_get_raw pkm pk)) (skey_get_raw pkm sk) (Plain.wire_t_to_bytesGT pkm.npm n)))
+    /\ ((dishonest pkm i \/ ~(b2t ae_ind_cpa)) ==>
+      (let repr_p = ((Plain.repr #pkm.pim #pkm.ppm #(compose_ids pkm (pkey_to_subId #pkm pk) (pkey_to_subId #pkm (pkey_from_skey pkm sk))) p)) in
+      (Plain.wire_t_to_bytesGT pkm.cpm c) == enc pkm (Plain.wire_t_to_bytesGT pkm.ppm repr_p) (Plain.wire_t_to_bytesGT pkm.pkpm (pkey_get_raw pkm pk)) (skey_get_raw pkm sk) (Plain.wire_t_to_bytesGT pkm.npm n)))
     // The message is added to the log. This also guarantees nonce-uniqueness.
     /\ MR.m_contains #(get_message_log_region pkm)(get_message_logGT pkm) h1
-    /\ MR.witnessed (MM.contains #(get_message_log_region pkm) (get_message_logGT pkm) (n,i) (c,m))
-    /\ MR.m_sel #(get_message_log_region pkm) h1 (get_message_logGT pkm)== MM.upd (MR.m_sel #(get_message_log_region pkm) h0 (get_message_logGT pkm)) (n,i) (c,m)
+    /\ MR.witnessed (MM.contains #(get_message_log_region pkm) (get_message_logGT pkm) ((Plain.wire_t_to_bytesGT pkm.npm n),i) ((Plain.wire_t_to_bytesGT pkm.cpm c),p))
+    /\ MR.m_sel #(get_message_log_region pkm) h1 (get_message_logGT pkm)== MM.upd (MR.m_sel #(get_message_log_region pkm) h0 (get_message_logGT pkm)) ((Plain.wire_t_to_bytesGT pkm.npm n),i) ((Plain.wire_t_to_bytesGT pkm.cpm c),p)
     /\ invariant pkm h1
   ))
 
 val decrypt: pkm:pkae_module ->
-             n:nonce ->
+             n:nonce pkm ->
              sk:skey pkm ->
              pk:pkey pkm{compatible_keys pkm sk pk} ->
-             c:cipher ->
-             ST (option (Plain.protected_plain_t pkm.pim (Plain.get_plain pkm.pm) (compose_ids pkm (pkey_to_subId #pkm pk) (pkey_to_subId #pkm (pkey_from_skey pkm sk)))))
+             c:cipher pkm ->
+             ST (option (protected_plain #pkm.pim #pkm.ppm (compose_ids pkm (pkey_to_subId #pkm pk) (pkey_to_subId #pkm (pkey_from_skey pkm sk)))))
   (requires (fun h0 ->
     let i = compose_ids pkm (pkey_to_subId #pkm pk) (pkey_to_subId #pkm (pkey_from_skey pkm sk)) in
     registered pkm i
@@ -151,21 +182,25 @@ val decrypt: pkm:pkae_module ->
   ))
   (ensures  (fun h0 p h1 ->
     let i = compose_ids pkm (pkey_to_subId #pkm pk) (pkey_to_subId #pkm (pkey_from_skey pkm sk)) in
-    h0 == h1
+    let nonce_bytes = Plain.wire_t_to_bytesGT pkm.npm n in
+    modifies_none h0 h1
     /\ invariant pkm h1
     /\ ((~(b2t pkae) \/ dishonest pkm i) ==> // Concrete behaviour of the id is dishonest or if the assumption doesn't hold.
-        (let option_m = dec pkm c n pk sk in // Functional correctness: we get a result iff the ciphertext is valid.
+        (let option_m = dec pkm (Plain.wire_t_to_bytesGT pkm.cpm c) (Plain.wire_t_to_bytesGT pkm.pkpm (pkey_get_raw pkm pk)) (skey_get_raw pkm sk) nonce_bytes in // Functional correctness: we get a result iff the ciphertext is valid.
         (Some? option_m ==>
-          Some? p /\ Some?.v p == Plain.make_prot_plainGT #pkm.pim #pkm.pm #i (Some?.v option_m))
+          Some? p
+          /\ (let v_option_m = Some?.v option_m in
+            let v_p = Some?.v p in
+            Plain.wire_t_to_bytesGT pkm.ppm (Plain.make_wire_tGT #pkm.pim #pkm.ppm #(compose_ids pkm (pkey_to_subId #pkm pk) (pkey_to_subId #pkm (pkey_from_skey pkm sk))) v_p) == v_option_m))
         /\ (None? option_m ==>
             None? p)
       ))
     /\ (let log = get_message_logGT pkm in
       (b2t pkae /\ honest pkm i) ==> // Ideal behaviour otherwise: We get a result iff something is in the log.
         (Some? p ==>
-          (MM.defined log (n,i) h0 /\ (fst (MM.value log (n,i) h0) == c )
-          /\ Some?.v p == snd (MM.value log (n,i) h0)))
+          (MM.defined log (nonce_bytes,i) h0 /\ (fst (MM.value log (nonce_bytes,i) h0) == (Plain.wire_t_to_bytesGT pkm.cpm c) )
+          /\ Some?.v p == snd (MM.value log (nonce_bytes,i) h0)))
       /\ (None? p ==>
-          (MM.fresh log (n,i) h0 \/ c =!= fst (MM.value log (n,i) h0)))
-    )
+          (MM.fresh log (nonce_bytes,i) h0 \/ Plain.wire_t_to_bytesGT pkm.cpm c =!= fst (MM.value log (nonce_bytes,i) h0)))
+      )
   ))
