secure_api/box/Box.Plain.fst
@@ -11,23 +11,71 @@ open FStar.HyperStack.ST
 open Box.Flags
 open Box.Index
 
+module Buffer = FStar.Buffer
+module Bytes = Crypto.Symmetric.Bytes
+
 (**
   The protected plaintext type of AE. It is associated with an id and acts as a wrapper around a protected pkae plaintext.
   The ids associated with both plaintexts must be equal.
 *)
 
 #set-options "--z3rlimit 300 --max_ifuel 1 --max_fuel 0"
+#set-options "--__temp_no_proj Box.Plain"
 abstract noeq type plain_module =
   | PM:
-    plain: Type0 ->
-    //repr: ((#i:id im) -> (protected_plain_t i) -> (p:plain_type{dishonest im (ID i) \/ not ae_ind_cpa})) ->
-    //coerce: (#i:id im -> plain_type -> (p:protected_plain_t i{dishonest im (ID i) \/ not ae_int_ctxt})) ->
-    valid_length: (nat -> bool)->
-    length: (plain -> n:nat{valid_length n}) ->
+    valid_length: (n:nat -> GTot (b:bool{n = 0 ==> false})) ->
     plain_module
+
+let plain (pm:plain_module) = buf:Buffer.buffer UInt8.t{pm.valid_length (Buffer.length buf)}
+let plain_bytes (pm:plain_module) = b:Bytes.bytes{pm.valid_length (Seq.length b)}
+
+val valid_length: pm:plain_module -> vl:(n:nat -> GTot (b:bool{n = 0 ==> false})){vl == pm.valid_length}
+let valid_length pm =
+  pm.valid_length
+
+val valid_plain_length: #pm:plain_module -> p:plain pm -> GTot (b:bool{b <==> pm.valid_length (Buffer.length p)})
+let valid_plain_length #pm p =
+  pm.valid_length (Buffer.length p)
 
 abstract type protected_plain_t (im:index_module) (pt:Type0) (id:id im) = pt
 
+(**
+  Allows changing from one protected type to another without breaking abstraction.
+*)
+val transmute_protected_plain_t: (#im:index_module) ->
+                               (#i:id im) ->
+                               (#pt1:Type0) ->
+                               (#pt2:Type0) ->
+                               (transmute:(pt1 -> pt2)) ->
+                               protected_plain_t im pt1 i ->
+                               protected_plain_t im pt2 i
+let transmute_protected_plain_t #im #i #pt1 #pt2 transmute p1 =
+  transmute p1
+
+(**
+  The same as transmute_protected_plain_t, just for stateful transmutation functions.
+*)
+val transmute_protected_plain_tST: (#im:index_module) ->
+                               (#i:id im) ->
+                               (#pt1:Type0) ->
+                               (#pt2:Type0) ->
+                               (transmute:(pt1 -> St (pt2))) ->
+                               protected_plain_t im pt1 i ->
+                               St (protected_plain_t im pt2 i)
+let transmute_protected_plain_tST #im #i #pt1 #pt2 transmute p1 =
+  transmute p1
+
+val live: #pm:plain_module -> p:plain pm -> h:mem -> t:Type0{t <==> Buffer.live h p}
+let live #pm p h = Buffer.live h p
+
+val plain_live: #im:index_module -> #pm:plain_module -> #id:id im -> p:protected_plain_t im (plain pm) id -> h:mem -> t:Type0{t <==> Buffer.live #UInt8.t h p}
+let plain_live #im #pm #id p h = Buffer.live #UInt8.t h p
+
+private val cast: #im:index_module -> #i:id im -> #a:Type0 -> p:(protected_plain_t im a i) -> a
+let cast #im #i #a p =
+  p
+
+#set-options "--z3rlimit 1000 --max_ifuel 2 --max_fuel 1"
 val lemma_index_module: im:index_module -> i:id im -> ST unit
   (requires (fun h0 -> registered im i))
   (ensures (fun h0 _ h1 ->
@@ -38,65 +86,118 @@ val lemma_index_module: im:index_module -> i:id im -> ST unit
 let lemma_index_module im i =
   lemma_index_module im i
 
-val get_plain: pm:plain_module -> (t:Type0{t == pm.plain})
-let get_plain pm =
-  pm.plain
-
-
-val make_plainGT: #im:index_module -> #pm:plain_module -> #i:id im -> protected_plain_t im pm.plain i -> GTot (p:pm.plain)
-let make_plainGT #im #pm #i p =
+val make_plain_tGT: #im:index_module -> #pm:plain_module -> #i:id im -> protected_plain_t im (plain pm) i -> GTot (p:plain pm)
+let make_plain_tGT #im #pm #i p =
   p
 
-val repr: #im:index_module -> #pm:plain_module -> #i:id im{dishonest im i \/ not ae_ind_cpa} -> protected_plain_t im pm.plain i -> (p:pm.plain)
+val protected_plain_length: #im:index_module -> #pm:plain_module -> #i:id im -> (p:protected_plain_t im (plain pm) i) -> GTot (n:nat{n==Buffer.length (cast p)})
+let protected_plain_length #im #pm #i p =
+  Buffer.length (cast p)
+
+val plain_length: #pm:plain_module -> len:(plain pm -> GTot nat){len == Buffer.length}
+let plain_length #pm = Buffer.length
+
+#set-options "--z3rlimit 1000 --max_ifuel 0 --max_fuel 0"
+val plain_to_bytesGT: #pm:plain_module -> wtb:(h:mem -> p:plain pm -> GTot (b:Bytes.bytes{Seq.length b == plain_length p}))
+let plain_to_bytesGT #pm =
+  FStar.Buffer.as_seq
+
+val plain_to_bytesST: #pm:plain_module -> p:plain pm -> STL (Seq.seq UInt8.t)
+  (requires (fun h0 -> Buffer.live h0 p))
+  (ensures (fun h0 b h1 ->
+    h0 == h1
+    /\ Buffer.live h1 p
+    /\ Seq.length b = plain_length p
+    /\ b == plain_to_bytesGT h1 p
+  ))
+let plain_to_bytesST #pm p =
+  FStar.Buffer.to_seq_full p
+
+#set-options "--z3rlimit 1000 --max_ifuel 1 --max_fuel 1"
+val bytes_to_plainST: pm:plain_module -> b:plain_bytes pm -> StackInline (p:plain pm)
+  (requires (fun h ->
+    0 < normalize_term (Seq.length b)
+    /\ normalize_term (Seq.length b) <= UInt.max_int 32
+  ))
+  (ensures (fun (h0:mem) p h1 ->
+     let len = plain_length p in
+     len > 0
+     /\ ~(Buffer.contains h0 p)
+     /\ Buffer.live h1 p /\ Buffer.idx p = 0 /\ plain_length p = len
+     /\ Buffer.frameOf p = h0.tip
+     /\ Map.domain h1.h == Map.domain h0.h
+     /\ Buffer.modifies_0 h0 h1
+     /\ plain_to_bytesGT h1 p == b
+   ))
+let bytes_to_plainST pm b =
+  let b_list = FStar.Seq.seq_to_list b in
+  let buf:plain pm = FStar.Buffer.createL b_list in
+  let b' = Seq.seq_of_list b_list in
+  Seq.lemma_seq_list_bij b;
+  buf
+
+// Not sure we can prove this with buffers...
+//val plain_t_to_bytes_inj_lemma: pm:plain_module -> w:pm.plain_t -> w':pm.plain_t -> Lemma
+//  (requires True)
+//  (ensures plain_t_to_bytesGT w == plain_t_to_bytesGT w' <==> w == w')
+//let plain_t_to_bytes_inj_lemma pm w w' =
+//  pm.plain_t_to_bytes_inj_lemma w w'
+
+#set-options "--z3rlimit 300 --max_ifuel 0 --max_fuel 0"
+val prot_length_lemma: #im:index_module -> #pm:plain_module -> #i:id im -> p:plain pm -> Lemma
+  (requires True)
+  (ensures
+    (let pp:protected_plain_t im (plain pm) i = p in
+    protected_plain_length pp  = plain_length p))
+  [SMTPat (protected_plain_length #im #pm #i p)]
+let prot_length_lemma #im #pm #i p = ()
+
+val repr: #im:index_module -> #pm:plain_module -> #i:id im{dishonest im i \/ not ae_ind_cpa} -> pp:protected_plain_t im (plain pm) i -> (p:plain pm{protected_plain_length pp = plain_length p})
 let repr #im #pm #i p =
   p
 
-val make_prot_plainGT: #im:index_module -> #pm:plain_module -> #i:id im -> p:pm.plain -> GTot (protected_plain_t im pm.plain i)
-let make_prot_plainGT #im #pm #i p =
+val make_prot_plain_tGT: #im:index_module -> #pm:plain_module -> #i:id im -> p:plain pm -> GTot (pp:protected_plain_t im (plain pm) i{protected_plain_length pp = plain_length p})
+let make_prot_plain_tGT #im #pm #i p =
   p
 
-val coerce: #im:index_module -> #pm:plain_module -> #i:id im{dishonest im i \/ not ae_int_ctxt} -> pm.plain -> (p:protected_plain_t im pm.plain i)
+val coerce: #im:index_module -> #pm:plain_module -> #i:id im{dishonest im i \/ not ae_int_ctxt} -> p:plain pm -> (pp:protected_plain_t im (plain pm) i{protected_plain_length pp = plain_length p})
 let coerce #im #pm #i p =
   p
 
-val valid_length: #pm:plain_module -> n:nat -> b:bool//{b=pm.valid_length n}
-let valid_length #pm n = pm.valid_length n
+//val lemma_valid_cipher_length: pm:plain_module -> Lemma (requires True) (ensures pm.valid_cipher_length == valid_cipher_length #pm) [SMTPat (valid_cipher_length #pm)]
+//let lemma_valid_cipher_length pm =
+//  assert (FStar.FunctionalExtensionality.feq (pm.valid_cipher_length) (valid_cipher_length #pm));
+//  ()
+//
+//val lemma_valid_plain_length: pm:plain_module -> Lemma (requires True) (ensures pm.valid_plain_length == valid_plain_length #pm) [SMTPat (valid_plain_length #pm)]
+//let lemma_valid_plain_length pm =
+//  assert (FStar.FunctionalExtensionality.feq (pm.valid_plain_length) (valid_plain_length #pm));
+//  ()
 
-val lemma_valid_length: pm:plain_module -> Lemma (requires True) (ensures pm.valid_length == valid_length #pm) [SMTPat (valid_length #pm)]
-let lemma_valid_length pm =
-  assert (FStar.FunctionalExtensionality.feq (pm.valid_length) (valid_length #pm));
-  ()
-
-val create: plain:Type0 ->
-            pm_valid_length:(nat -> bool) ->
-            length:(plain ->
-            n:nat{pm_valid_length n}) ->
+#set-options "--z3rlimit 1000 --max_ifuel 2 --max_fuel 1"
+val create: pm_valid_length: (n:nat -> GTot (b:bool{n = 0 ==> false})) ->
             pm:plain_module{
-              pm.plain==plain
-              /\ get_plain pm == plain
-              /\ valid_length #pm == pm_valid_length
-              /\ pm.valid_length == pm_valid_length
-              /\ pm.length==length}
-let create plain valid_length length =
-  PM plain valid_length length
+              pm.valid_length == pm_valid_length
+              }
 
-val length: #im:index_module -> #pm:plain_module -> #i:id im -> (p:protected_plain_t im pm.plain i) -> n:nat{n=pm.length p /\ pm.valid_length n}
-let length #im #pm #i p =
-  pm.length p
+let create valid_length =
+  PM valid_length
 
-val rec_repr: #im:index_module ->
-              #inner_pm:plain_module ->
-              #pm:plain_module ->
-              #i:id im{dishonest im i \/ not ae_ind_cpa} ->
-              p:protected_plain_t im pm.plain i{protected_plain_t im pm.plain i === protected_plain_t im inner_pm.plain i}
-              -> Tot (inner_pm.plain)
-let rec_repr #im #inner_pm #pm #i p =
-  repr #im #inner_pm #i p
+// We probably don't need this anymore, as plain modules are much simpler now.
+//val rec_repr: #im:index_module ->
+//              #inner_pm:plain_module ->
+//              #pm:plain_module ->
+//              #i:id im{dishonest im i \/ not ae_ind_cpa} ->
+//              p:protected_plain_t im (plain pm) i
+//              -> Tot (plain inner_pm)
+//let rec_repr #im #inner_pm #pm #i p =
+//  assume(protected_plain_t im (plain pm) i == protected_plain_t im (plain inner_pm) i);
+//  repr #im #inner_pm #i p
 
-val message_wrap: #im:index_module -> #inner_pm:plain_module -> #pm:plain_module -> #i:id im -> p:inner_pm.plain{protected_plain_t im pm.plain i === protected_plain_t im inner_pm.plain i} -> protected_plain_t im pm.plain i
+val message_wrap: #im:index_module -> #inner_pm:plain_module -> #pm:plain_module -> #i:id im -> p:plain inner_pm{protected_plain_t im (plain pm) i === protected_plain_t im (plain inner_pm) i} -> protected_plain_t im (plain pm) i
 let message_wrap #im #inner_pm #pm #i p =
   p
 
-val message_unwrap: #im:index_module -> #inner_pm:plain_module -> #pm:plain_module -> #i:id im -> p:pm.plain{protected_plain_t im pm.plain i === protected_plain_t im inner_pm.plain i} -> protected_plain_t im inner_pm.plain i
+val message_unwrap: #im:index_module -> #inner_pm:plain_module -> #pm:plain_module -> #i:id im -> p:(plain pm){protected_plain_t im (plain pm) i === protected_plain_t im (plain inner_pm) i} -> protected_plain_t im (plain inner_pm) i
 let message_unwrap #im #inner_pm #pm #i p =
   p
