secure_api/box/Box.AE.fsti
@@ -1,0 +1,282 @@
+module Box.AE
+
+open FStar.Set
+open FStar.HyperHeap
+open FStar.HyperStack
+open FStar.HyperStack.ST
+open FStar.Monotonic.RRef
+
+open Crypto.Symmetric.Bytes
+
+open Box.Flags
+open Box.Plain
+open Box.Index
+open Box.Key
+
+module MR = FStar.Monotonic.RRef
+module HH = FStar.HyperHeap
+module HS = FStar.HyperStack
+module MM = MonotoneMap
+module Plain = Box.Plain
+module Key = Box.Key
+module ID = Box.Index
+
+// Some basic types
+val key_t: (pm:plain_module) -> (im:index_module) -> i:id im -> Type0
+
+let log_region =
+  r:MR.rid{is_eternal_region r}
+
+let protected_plain (#im:index_module) (#pm:plain_module) (i:id im) = p:Plain.protected_plain_t im (pt:plain pm) i{Plain.valid_plain_length (Plain.make_plain_tGT p)}
+let plain_bytes (#pm:plain_module) = b:bytes{Plain.valid_length pm (Seq.length b)}
+
+// Key log types
+let key_log_key (im:index_module) = i:id im
+let key_log_value (kpm:plain_module) (im:index_module) (i:id im) = (key_t kpm im i)
+let key_log_range (kpm:plain_module) (im:index_module) = fun (k:key_log_key im) -> (v:key_log_value kpm im k)
+let key_log_inv (kpm:plain_module) (im:index_module) (f:MM.map' (key_log_key im) (key_log_range kpm im)) = True
+
+let key_log_t (kpm:plain_module) (im:index_module) (rgn:log_region) = MM.t rgn (key_log_key im) (key_log_range kpm im) (key_log_inv kpm im)
+
+
+// Message log types
+let message_log_key (im:index_module) (npm:plain_module) = (plain_bytes #npm*(i:id im))
+let message_log_value (im:index_module) (cpm:plain_module) (ppm:plain_module) (i:id im) = (c:plain_bytes #cpm*m:protected_plain #im #ppm i)
+let message_log_range (im:index_module) (cpm:plain_module) (ppm:plain_module) (npm:plain_module) (k:message_log_key im npm) = (message_log_value im cpm ppm (snd k))
+let message_log_inv (im:index_module) (cpm:plain_module) (ppm:plain_module) (npm:plain_module) (f:MM.map' (message_log_key im npm) (message_log_range im cpm ppm npm)) = True
+
+let message_log (im:index_module) (cpm:plain_module) (ppm:plain_module) (npm:plain_module) (rgn:log_region) =
+  MM.t rgn (message_log_key im npm) (message_log_range im cpm ppm npm) (message_log_inv im cpm ppm npm)
+
+#set-options "--__temp_no_proj Box.AE"
+abstract noeq type ae_module (im:index_module) =
+  | AM :
+    key_length: UInt32.t{(UInt32.v key_length) > 0} ->
+    ppm:plain_module ->
+    cpm:plain_module ->
+    kpm:plain_module{Plain.valid_length kpm == (Key.check_length (UInt32.v key_length))} ->
+    npm:plain_module ->
+    compute_cipher_length: (plain_len:nat{Plain.valid_length ppm plain_len} -> cipher_len:nat{Plain.valid_length cpm cipher_len}) ->
+    compute_plain_length:  (cipher_len:nat{Plain.valid_length cpm cipher_len} -> plain_len:nat{Plain.valid_length ppm plain_len}) ->
+    enc: (p:plain_bytes #ppm -> plain_bytes #kpm -> plain_bytes #npm -> Tot (c:bytes{Seq.length c = compute_cipher_length (Seq.length p)})) ->
+    dec: (c:plain_bytes #cpm -> plain_bytes #kpm -> plain_bytes #npm -> Tot (option (p:bytes{Seq.length p = compute_plain_length (Seq.length c)}))) ->
+    enc_low:(p:plain ppm -> k:plain kpm -> n:plain npm -> ST (c:plain cpm)
+      (requires (fun h0 -> True))
+      (ensures (fun h0 c h1 ->
+        Plain.plain_to_bytesGT h1 c == enc (Plain.plain_to_bytesGT h1 p) (Plain.plain_to_bytesGT h1 k) (Plain.plain_to_bytesGT h1 n)
+        /\ modifies_none h0 h1
+        /\ Plain.live c h1
+      ))
+      ) ->
+    dec_low:(c:plain cpm -> k:plain kpm -> n:plain npm -> ST (option (p:plain ppm))
+      (requires (fun h0 -> True))
+      (ensures (fun h0 p h1 ->
+        let spec_p = dec (Plain.plain_to_bytesGT h1 c) (Plain.plain_to_bytesGT h1 k) (Plain.plain_to_bytesGT h1 n) in
+        (Some? p ==> (let v = Some?.v p in
+          Some? spec_p /\ Plain.plain_to_bytesGT h1 v == Some?.v spec_p /\ Plain.live (Some?.v p) h1))
+        /\ (None? p ==> None? spec_p)
+        /\ modifies_none h0 h1
+      ))
+      ) ->
+    key_log_region: (rgn:log_region{disjoint rgn (ID.get_rgn im) /\ is_eternal_region rgn})->
+    message_log_region: (rgn:log_region{disjoint rgn key_log_region /\ disjoint rgn (ID.get_rgn im) /\ is_eternal_region rgn}) ->
+    key_log: (key_log_t kpm im key_log_region) ->
+    message_log: (message_log im cpm ppm npm message_log_region) ->
+    ae_module im
+
+let cipher (#im:index_module) (am:ae_module im) = (c:Plain.plain am.cpm)
+//let plain  (#im:index_module) (am:ae_module im) = (p:Plain.plain am.ppm)
+let nonce (#im:index_module) (am:ae_module im) = (n:Plain.plain am.npm )
+let nonce_bytes (#im:index_module) (am:ae_module im) = (n:Plain.plain_bytes am.npm )
+let key (#im:index_module) (#am:ae_module im) (i:id im) = key_t am.kpm im i
+let key_raw (#im:index_module) (#am:ae_module im) = raw_t:plain_bytes #am.kpm
+
+val create_zero_bytes: n:nat -> Tot (b:bytes{b=Seq.create n (UInt8.uint_to_t 0)})
+
+private val get_rawGT: #im:index_module -> #am:ae_module im -> i:id im -> k:key #im #am i -> GTot (key_raw #im #am)
+
+val recall_logs: #im:index_module -> am:ae_module im -> ST unit
+  (requires (fun h0 -> True))
+  (ensures (fun h0 _ h1 ->
+    h0 == h1
+    /\ MR.m_contains am.message_log h1
+    /\ MR.m_contains am.key_log h1
+  ))
+
+val get_message_log_region: #im:index_module  -> am:ae_module im -> Tot (lr:log_region{lr == am.message_log_region})
+
+#set-options "--__temp_no_proj Box.AE"
+#set-options "--z3rlimit 200 --max_ifuel 1 --max_fuel 0"
+val get_message_logGT: #im:index_module  -> am:ae_module im -> Tot (ml:message_log im am.cpm am.ppm am.npm am.message_log_region{ml == am.message_log})
+
+val get_ppm: #im:index_module -> am:ae_module im -> pm:plain_module{pm == am.ppm}
+val get_cpm: #im:index_module -> am:ae_module im -> pm:plain_module{pm == am.cpm}
+val get_npm: #im:index_module -> am:ae_module im -> pm:plain_module{pm == am.npm}
+val get_kpm: #im:index_module -> am:ae_module im -> pm:plain_module{pm == am.kpm}
+
+val compute_cipher_length: (#im:index_module) -> (am:ae_module im) -> (plain_len:nat{Plain.valid_length am.ppm plain_len} -> cipher_len:nat{Plain.valid_length am.cpm cipher_len})
+val compute_plain_length: (#im:index_module) -> (am:ae_module im) -> (cipher_len:nat{Plain.valid_length am.cpm cipher_len} -> plain_len:nat{Plain.valid_length am.ppm plain_len})
+
+val nonce_is_fresh: (#im:index_module) -> (am:ae_module im) -> (i:id im) -> (n:nonce_bytes am) -> (h:mem) -> (t:Type0{t <==>
+    (MR.m_contains am.message_log h
+    /\ MM.fresh am.message_log (n,i) h)})
+
+let log_freshness_invariant (#im:index_module) (am:ae_module im) (h:mem) =
+  MR.m_contains (get_log im) h
+  /\ MR.m_contains am.message_log h
+  /\ (forall i n . ID.fresh im i h ==> MM.fresh am.message_log (n,i) h)
+
+//val log_freshness_framing_lemma: #im:index_module -> am:ae_module im -> h0:mem -> h1:mem -> Lemma
+//  (requires log_freshness_invariant am h0)
+//  (ensures (modifies_none h0 h1 ==> (log_freshness_invariant am h1)))
+
+val lemma_nonce_freshness: #im:index_module  -> am:ae_module im -> i:id im -> n:nonce_bytes am -> h0:mem -> h1:mem -> Lemma
+  (requires nonce_is_fresh am i n h0 /\ (modifies (Set.singleton am.key_log_region) h0 h1 \/ h0 == h1))
+  (ensures ((modifies (Set.singleton am.key_log_region) h0 h1 \/ h0 == h1) ==> nonce_is_fresh am i n h1))
+
+val create: im:index_module ->
+            rgn:log_region{disjoint rgn (ID.get_rgn im) /\ is_just_below root rgn} ->
+            key_length: UInt32.t{(UInt32.v key_length > 0)} ->
+            ppm:plain_module ->
+            cpm:plain_module ->
+            kpm:plain_module{Plain.valid_length kpm == (check_length (UInt32.v key_length))} ->
+            npm:plain_module ->
+            compute_cipher_length: (plain_len:nat{Plain.valid_length ppm plain_len} -> cipher_len:nat{Plain.valid_length cpm cipher_len}) ->
+            compute_plain_length:  (cipher_len:nat{Plain.valid_length cpm cipher_len} -> plain_len:nat{Plain.valid_length ppm plain_len}) ->
+            enc: (p:plain_bytes #ppm -> plain_bytes #kpm -> plain_bytes #npm -> Tot (c:bytes{Seq.length c = compute_cipher_length (Seq.length p)})) ->
+            dec: (c:plain_bytes #cpm -> plain_bytes #kpm -> plain_bytes #npm -> Tot (option (p:bytes{Seq.length p = compute_plain_length (Seq.length c)}))) ->
+            enc_low:(p:plain ppm -> k:plain kpm -> n:plain npm -> ST (c:plain cpm)
+              (requires (fun h0 -> True))
+              (ensures (fun h0 c h1 ->
+                Plain.plain_to_bytesGT h1 c == enc (Plain.plain_to_bytesGT h1 p) (Plain.plain_to_bytesGT h1 k) (Plain.plain_to_bytesGT h1 n)
+                /\ modifies_none h0 h1
+                /\ Plain.live c h1
+              ))
+              ) ->
+            dec_low:(c:plain cpm -> k:plain kpm -> n:plain npm -> ST (option (p:plain ppm))
+              (requires (fun h0 -> True))
+              (ensures (fun h0 p h1 ->
+                let spec_p = dec (Plain.plain_to_bytesGT h1 c) (Plain.plain_to_bytesGT h1 k) (Plain.plain_to_bytesGT h1 n) in
+                (Some? p ==> (let v = Some?.v p in
+                  Some? spec_p /\ Plain.plain_to_bytesGT h1 v == Some?.v spec_p /\ Plain.live (Some?.v p) h1))
+                /\ (None? p ==> None? spec_p)
+                /\ modifies_none h0 h1
+              ))
+              ) ->
+            ST (am:ae_module im)
+  (requires (fun h0 ->
+    True
+  ))
+  (ensures (fun h0 am h1 ->
+    modifies_none h0 h1
+    /\ HH.extends am.message_log_region rgn
+    /\ HH.extends am.key_log_region rgn
+    /\ disjoint am.message_log_region am.key_log_region
+    /\ MR.m_contains am.key_log h1
+    /\ MR.m_contains am.message_log h1
+    /\ MR.m_sel #am.key_log_region h1 am.key_log == MM.empty_map (key_log_key im) (key_log_range kpm im)
+    /\ MR.m_sel #am.message_log_region h1 am.message_log == MM.empty_map (message_log_key im am.npm) (message_log_range im am.cpm am.ppm am.npm)
+    /\ log_freshness_invariant #im am h1
+    /\ ppm == am.ppm
+    /\ cpm == am.cpm
+    /\ kpm == am.kpm
+    /\ npm == am.npm
+  ))
+
+private val gen: #im:index_module  -> #am:ae_module im -> i:id im -> ST (k:key #im #am i)
+  (requires (fun h0 ->
+    (fresh im i h0 \/ honest im i)
+    /\ log_freshness_invariant am h0
+  ))
+  (ensures  (fun h0 k h1 ->
+    (MM.fresh am.key_log i h0 ==>
+              (modifies (Set.singleton am.key_log_region) h0 h1
+              /\ MR.m_sel h1 am.key_log == MM.upd (MR.m_sel h0 am.key_log) i k))
+    /\ (MM.defined am.key_log i h0 ==> h0 == h1)
+    /\ log_freshness_invariant am h1
+  ))
+
+private val set: #im:index_module -> #am:ae_module im -> i:id im{~(Game2? current_game)} -> raw:key_raw #im #am -> (k:key #im #am i{get_rawGT i k == raw})
+
+private val coerce: #im:index_module -> #am:ae_module im -> i:id im{dishonest im i} -> raw:key_raw #im #am -> (k:key #im #am i{get_rawGT i k == raw})
+
+private val leak: #im:index_module -> #am:ae_module im -> i:id im{dishonest im i} -> k:key #im #am i -> Tot (raw:key_raw #im #am{raw == get_rawGT i k})
+
+val instantiate_km: #im:index_module -> am:ae_module im -> km:key_module im{
+    Key.get_keylen km == (UInt32.v am.key_length)
+    /\ Key.get_pm km == am.kpm
+    /\ Key.get_keytype km == key #im #am
+    /\ Key.get_rawGT km == get_rawGT #im #am
+    /\ Key.invariant km == log_freshness_invariant am
+    /\ Key.get_log_region km == am.key_log_region
+    /\ disjoint (Key.get_log_region km) am.message_log_region
+    }
+
+#reset-options
+(**
+   Encrypt a a message under a key. Idealize if the key is honest and ae_ind_cca true.
+*)
+ #set-options "--z3rlimit 500 --max_ifuel 1 --max_fuel 0"
+val encrypt: #im:index_module -> am:ae_module im -> #(i:id im) -> nl:nat{Plain.valid_length am.npm nl} -> n:nonce am{Plain.plain_length #am.npm n = nl} -> k:key #im #am i -> pl:nat{Plain.valid_length am.ppm pl} -> p:protected_plain #im #am.ppm i{Plain.protected_plain_length #im #am.ppm p = pl} -> c:cipher am -> StackInline unit
+(requires (fun h0 ->
+  registered im i
+  /\ nonce_is_fresh #im am i (Plain.plain_to_bytesGT h0 n) h0 // Nonce freshness
+  /\ log_freshness_invariant #im am h0
+  /\ Plain.plain_live p h0
+  /\ Plain.live n h0
+  /\ Plain.live c h0
+))
+(ensures  (fun h0 _ h1 ->
+  registered im i
+  /\ modifies (Set.singleton (get_message_log_region #im am)) h0 h1 // stateful changes even if the id is dishonest.
+  /\ ((honest im i /\ b2t ae_ind_cpa) // Ideal behaviour if the id is honest and the assumption holds.
+      ==> ((Plain.plain_to_bytesGT h1 c) == am.enc (create_zero_bytes (Plain.protected_plain_length #im #am.ppm #i p)) (get_rawGT i k) (Plain.plain_to_bytesGT h1 n)))
+  /\ ((dishonest im i \/ ~(b2t ae_ind_cpa)) ==>
+      (let repr_p = ((Plain.repr #im #am.ppm #i p)) in
+      (Plain.plain_to_bytesGT h1 c) == am.enc (Plain.plain_to_bytesGT h1 repr_p) (get_rawGT i k) (Plain.plain_to_bytesGT h1 n)))
+  /\ MR.m_contains am.message_log h1  // A message is added to the log even if the id is dishonest. This also guarantees nonce-uniqueness.
+  /\ MR.witnessed (MM.contains am.message_log ((Plain.plain_to_bytesGT h1 n),i) ((Plain.plain_to_bytesGT h1 c),p))
+  /\ MR.m_sel h1 am.message_log == MM.upd (MR.m_sel h0 am.message_log) ((Plain.plain_to_bytesGT h1 n),i) ((Plain.plain_to_bytesGT h1 c),p)
+  /\ log_freshness_invariant #im am h1
+  /\ Plain.live c h1
+  /\ Plain.plain_live p h1
+))
+
+(**
+   Decrypt a ciphertext c using a key k. If the key is honest and ae_int_ctxt is idealized,
+   try to obtain the ciphertext from the log. Else decrypt via concrete implementation.
+*)
+//#set-options "--z3rlimit 1000 --max_ifuel 1 --max_fuel 0"
+val decrypt: #im:index_module -> am:ae_module im -> #(i:id im) -> nl:nat{Plain.valid_length am.npm nl} ->  n:nonce am{Plain.plain_length #am.npm n = nl} -> k:key #im #am i -> cl:nat{Plain.valid_length am.ppm cl} -> c:cipher am{Plain.plain_length #am.cpm c = cl} -> StackInline (option (protected_plain #im #am.ppm i))
+  (requires (fun h0 ->
+    registered im i // No in-between states of keys (i.e.) where one of the shares is fresh and one is registered
+    /\ Plain.live c h0
+    /\ Plain.live n h0
+  ))
+  (ensures  (fun h0 p h1 ->
+    let modified_regions_honest = Set.singleton am.message_log_region in
+    let byte_nonce = Plain.plain_to_bytesGT h1 n in
+    registered im i
+    /\ modifies_none h0 h1
+    /\ ((~(b2t ae_int_ctxt) \/ dishonest im i) ==> // Concrete behaviour of the id is dishonest or if the assumption doesn't hold.
+        (let option_m = am.dec (Plain.plain_to_bytesGT h1 c) (get_rawGT i k) byte_nonce in // Functional correctness: we get a result iff the ciphertext is valid.
+          (Some? option_m ==>
+            (Some? p
+            /\ (let v_option_m = Some?.v option_m in
+              let v_p = Some?.v p in
+              (Plain.plain_to_bytesGT h1 (Plain.make_plain_tGT #im #am.ppm #i v_p)) == v_option_m
+              /\ Plain.plain_live #im #am.ppm #i v_p h1)))
+          /\ (None? option_m ==>
+              None? p)
+      ))
+    // Ideal behaviour otherwise: We get a result iff something is in the log.
+    /\ ((b2t ae_int_ctxt /\ honest im i) ==>
+        (Some? p ==>
+          (let v = Some?.v p in
+          MM.defined am.message_log (byte_nonce,i) h0 /\ (fst (MM.value am.message_log (byte_nonce,i) h0) == (Plain.plain_to_bytesGT h1 c))
+          /\ v == snd (MM.value am.message_log (byte_nonce,i) h0)
+          /\ Plain.plain_live #im #am.ppm #i v h1))
+    /\ (None? p
+    ==> (MM.fresh am.message_log (byte_nonce,i) h0 \/ (Plain.plain_to_bytesGT h1 c) =!= fst (MM.value am.message_log (byte_nonce,i) h0)))
+   )
+  ))
